theories/Eq/UpToTaus.v
@@ -27,364 +27,59 @@ From Coq Require Import
      Relations.Relations.
 
 From ITree Require Import
-     Core.
+     Core
+     UpToTausExplicit.
 
 From ITree Require Export
      Eq.Eq.
 
 Local Open Scope itree.
 
-Section FiniteTaus.
-
-Context {E : Type -> Type} {R : Type}.
-
-(* [notau t] holds when [t] does not start with a [Tau]. *)
-Definition notauF {I} (t : itreeF E R I) : Prop :=
-  match t with
-  | TauF _ => False
-  | _ => True
-  end.
-
-Notation notau t := (notauF (observe t)).
-
-(* [untaus t t'] holds when [t = Tau (... Tau t' ...)]:
-   [t] steps to [t'] by "peeling off" a finite number of [Tau].
-   "Peel off" means to remove only taus at the root of the tree,
-   not any behind a [Vis] step). *)
-Inductive untausF :
-  itreeF E R (itree E R) -> itreeF E R (itree E R) -> Prop :=
-| NoTau ot0 : untausF ot0 ot0
-| OneTau ot t' ot0 (OBS: TauF t' = ot) (TAUS: untausF (observe t') ot0): untausF ot ot0
-.
-Hint Constructors untausF.
-
-Definition unalltausF ot ot0 := untausF ot ot0 /\ notauF ot0.
-Hint Unfold unalltausF.
-
-Lemma unalltausF_untausF ot ot0 : unalltausF ot ot0 -> untausF ot ot0.
-Proof. intros []; auto. Qed.
-Hint Resolve unalltausF_untausF.
-
-Lemma unalltausF_notauF ot ot0 : unalltausF ot ot0 -> notauF ot0.
-Proof. intros []; auto. Qed.
-Hint Resolve unalltausF_notauF.
-
-(* [finite_taus t] holds when [t] has a finite number of taus
-   to peel. *)
-Definition finite_tausF ot : Prop := exists ot', unalltausF ot ot'.
-Hint Unfold finite_tausF.
-
-(** ** Lemmas *)
-
-Lemma untaus_all ot ot' :
-  untausF ot ot' -> notauF ot' -> unalltausF ot ot'.
-Proof. induction 1; eauto. Qed.
-
-Lemma unalltaus_notau ot ot' : unalltausF ot ot' -> notauF ot'.
-Proof. intros. induction H; eauto. Qed.
-
-Lemma notau_tau I (ot : itreeF E R I) (t0 : I)
-  (NOTAU : notauF ot)
-  (OBS: TauF t0 = ot): False.
-Proof. subst. auto. Qed.
-Hint Resolve notau_tau.
-
-Lemma notau_ret I (ot: itreeF E R I) r (OBS: RetF r = ot) : notauF ot.
-Proof. subst. red. eauto. Qed.
-Hint Resolve notau_ret.
-
-Lemma notau_vis I (ot : itreeF E R I) u (e: E u) k (OBS: VisF e k = ot) : notauF ot.
-Proof. intros. subst. red. eauto. Qed.
-Hint Resolve notau_vis.
-
-(* If [t] does not start with [Tau], removing all [Tau] does
-   nothing. Can be thought of as [notau_unalltaus] composed with
-   [unalltaus_injective] (below). *)
-Lemma unalltaus_notau_id ot ot' :
-  unalltausF ot ot' -> notauF ot -> ot = ot'.
-Proof.
-  intros [[ | ]] ?; eauto. exfalso; eauto.
-Qed.
-
-(* There is only one way to peel off all taus. *)
-Lemma unalltaus_injective ot ot1 ot2 :
-    unalltausF ot ot1 -> unalltausF ot ot2 -> ot1 = ot2.
-Proof.
-  intros [Huntaus Hnotau]. revert ot2 Hnotau.
-  induction Huntaus; intros; eauto using unalltaus_notau_id.
-  eapply IHHuntaus; eauto.
-  destruct H as [Huntaus' Hnotau'].
-  destruct Huntaus'.
-  + exfalso; eauto.
-  + subst. inversion OBS0; subst; eauto.
-Qed.
-
-(* Adding a [Tau] to [t1] then peeling them all off produces
-   the same result as peeling them all off from [t1]. *)
-Lemma unalltaus_tau t ot1 ot2
-    (OBS: TauF t = ot1)
-    (TAUS: unalltausF ot1 ot2):
-  unalltausF (observe t) ot2.
-Proof.
-  destruct TAUS as [Huntaus Hnotau].
-  destruct Huntaus.
-  - exfalso; eauto.
-  - subst; inversion OBS0; subst; eauto.
-Qed.
-
-Lemma unalltaus_tau' t ot1 ot2
-    (OBS: TauF t = ot1)
-    (TAUS: unalltausF (observe t) ot2):
-  unalltausF ot1 ot2.
-Proof.
-  destruct TAUS as [Huntaus Hnotau].
-  subst. eauto.
-Qed.
-
-Lemma notauF_untausF ot1 ot2
-      (NOTAU : notauF ot1)
-      (UNTAUS : untausF ot1 ot2) : ot1 = ot2.
-Proof.
-  destruct UNTAUS; eauto.
-  exfalso; eauto.
-Qed.
-
-Definition untausF_shift (t1 t2 : itree E R) :
-  untausF (TauF t1) (TauF t2) -> untausF (observe t1) (observe t2).
-Proof.
-  intros H.
-  inversion H; subst.
-  { constructor. }
-  clear H.
-  inversion OBS; subst; clear OBS.
-  remember (observe t1) as ot1.
-  remember (TauF t2) as tt2.
-  generalize dependent t1.
-  generalize dependent t2.
-  induction TAUS; intros; subst; econstructor; eauto.
-Qed.
-
-Definition untausF_trans (t1 t2 t3 : itreeF E R _) :
-  untausF t1 t2 -> untausF t2 t3 -> untausF t1 t3.
-Proof.
-  induction 1; auto.
-  subst; econstructor; auto.
-Qed.
-
-Definition untausF_strong_ind
-           (P : itreeF E R _ -> Prop)
-           (ot1 ot2 : itreeF E R _)
-           (Huntaus : untausF ot1 ot2)
-           (Hnotau : notauF ot2)
-           (STEP : forall ot1
-               (Huntaus : untausF ot1 ot2)
-               (IH: forall t1' oti
-                     (NEXT: ot1 = TauF t1')
-                     (UNTAUS: untausF (observe t1') oti),
-                   P oti),
-               P ot1)
-  : P ot1.
-Proof.
-  enough (H : forall oti,
-             untausF ot1 oti ->
-             untausF oti ot2 ->
-             P oti
-         ).
-  { apply H; eauto. }
-  revert STEP.
-  induction Huntaus; intros; subst.
-  - eapply STEP; eauto.
-    intros; subst. dependent destruction H; inv Hnotau.
-  - destruct H0; auto.
-    subst. apply STEP; eauto.
-    intros. inv NEXT.
-    apply IHHuntaus; eauto.
-    + clear -H UNTAUS.
-      remember (TauF t') as ott'. remember (TauF t1') as ott1'.
-      move H at top. revert_until H. induction H; intros; subst.
-      * inv Heqott1'. eauto.
-      * inv Heqott'. dependent destruction H; eauto.
-    + genobs t1' ot1'. revert UNTAUS. clear -Hnotau H0. induction H0; intros.
-      * dependent destruction UNTAUS; eauto.
-        subst. simpobs. inv Hnotau.
-      * subst. dependent destruction UNTAUS; eauto.
-Qed.
-
-(* If [t] does not start with [Tau], then it starts with finitely
-   many [Tau]. *)
-Lemma notau_finite_taus ot : notauF ot -> finite_tausF ot.
-Proof. eauto. Qed.
-
-(* [Vis] and [Ret] start with no taus, of course. *)
-Lemma finite_taus_ret ot (r : R) (OBS: RetF r = ot) : finite_tausF ot.
-Proof. eauto 10. Qed.
-
-Lemma finite_taus_vis {u} ot (e : E u) (k : u -> itree E R) (OBS: VisF e k = ot):
-  finite_tausF ot.
-Proof. eauto 10. Qed.
-
-(* [finite_taus] is preserved by removing or adding one [Tau]. *)
-Lemma finite_taus_tau t':
-  finite_tausF (TauF t') <-> finite_tausF (observe t').
-Proof.
-  split; intros [? [Huntaus Hnotau]]; eauto 10.
-  inv Huntaus.
-  - contradiction.
-  - inv OBS; eauto.
-Qed.
-
-(* (* [finite_taus] is preserved by removing or adding any finite *)
-(*    number of [Tau]. *) *)
-Lemma untaus_finite_taus ot ot':
-    untausF ot ot' -> (finite_tausF ot <-> finite_tausF ot').
-Proof.
-  induction 1; intros; subst.
-  - reflexivity.
-  - erewrite finite_taus_tau; eauto.
-Qed.
-
-Lemma untaus_untaus : forall (ot1 ot2 ot3: itreeF E R _),
-    untausF ot1 ot2 -> untausF ot2 ot3 -> untausF ot1 ot3.
-Proof.
-  intros t1 t2 t3. induction 1; simpl; eauto.
-Qed.
-
-Lemma untaus_unalltaus_rev (ot1 ot2 ot3: itreeF E R _) :
-    untausF ot1 ot2 -> unalltausF ot1 ot3 -> unalltausF ot2 ot3.
-Proof.
-  intros H. revert ot3.
-  induction H; intros.
-  - eauto with arith.
-  - destruct H0 as [Huntaus Hnotau].
-    destruct Huntaus.
-    + exfalso; eauto.
-    + inv OBS0. inversion H0; subst; eauto.
-Qed.
-
-Lemma unalltausF_ret : forall x (t: itree' E R),
-    unalltausF (RetF x) t -> t = RetF x.
-Proof.
-  intros x t [UNT NOT]; inversion UNT; subst; clear UNT; [reflexivity | easy].
-Qed.
-
-Lemma unalltausF_vis {S}: forall e (k: S -> itree E R) (t: itree' E R),
-    unalltausF (VisF e k) t -> t = VisF e k.
-Proof.
-  intros e k t [UNT NOT]; inversion UNT; subst; clear UNT; [reflexivity | easy].
-Qed.
-
-End FiniteTaus.
-
-Arguments untaus_unalltaus_rev : clear implicits.
-
-Hint Resolve unalltausF_notauF.
-Hint Resolve unalltausF_untausF.
-
-Hint Constructors untausF.
-Hint Unfold unalltausF.
-Hint Unfold finite_tausF.
-Hint Resolve notau_ret.
-Hint Resolve notau_vis.
-Hint Resolve notau_tau.
-
-Notation finite_taus t := (finite_tausF (observe t)).
-Notation untaus t t' := (untausF (observe t) (observe t')).
-Notation unalltaus t t' := (unalltausF (observe t) (observe t')).
-
-Ltac auto_untaus :=
-  repeat match goal with
-  | [ H1 : notauF ?X, H2 : unalltausF ?X ?Y |- _ ] =>
-    assert_fails (unify X Y);
-    replace Y with X in * by apply (unalltaus_notau_id _ _ H2 H1)
-  | [ H1 : unalltausF ?X ?Y, H2 : unalltausF ?X ?Z |- _ ] =>
-    assert_fails (unify Y Z);
-    replace Z with Y in * by apply (unalltaus_injective _ _ _ H1 H2)
-  end; auto.
 
 Section EUTT.
 
 Context {E : Type -> Type} {R1 R2 : Type} (RR : R1 -> R2 -> Prop).
 
-(* Equivalence between visible steps of computation (i.e., [Vis] or
-   [Ret], parameterized by a relation [eutt] between continuations
-   in the [Vis] case. *)
-Variant eq_notauF {I J} (eutt : I -> J -> Prop)
-: itreeF E R1 I -> itreeF E R2 J -> Prop :=
-| Eutt_ret : forall r1 r2,
-    RR r1 r2 ->
-    eq_notauF eutt (RetF r1) (RetF r2)
-| Eutt_vis : forall u (e : E u) k1 k2,
-    (forall x, eutt (k1 x) (k2 x)) ->
-    eq_notauF eutt (VisF e k1) (VisF e k2).
-Hint Constructors eq_notauF.
-
-Lemma eq_notauF_vis_inv1 {I J} {eutt : I -> J -> Prop} {U}
-  ot (e : E U) k :
-  eq_notauF eutt ot (VisF e k) ->
-  exists k',
-    ot = VisF e k' /\ (forall x, eutt (k' x) (k x)).
-Proof.
-  intros. remember (VisF e k) as t.
-  inversion H; subst; try discriminate.
-  inversion H2; subst; auto_inj_pair2; subst; eauto.
-Qed.
-
-(*
-Variant eq_notauF' {I} (eutt : relation I)
-: relation (itreeF E R I) :=
-| Eutt_ret' : forall r, eq_notauF' eutt (RetF r) (RetF r)
-| Eutt_vis' : forall {u1 u2} (e1 : E u1) (e2 : E u2) k1 k2,
-    eq_dep _ E _ e1 _ e2 ->
-    (forall x1 x2, JMeq x1 x2 -> eutt (k1 x1) (k2 x2)) ->
-    eq_notauF' eutt (VisF e1 k1) (VisF e2 k2).
-Hint Constructors eq_notauF'.
-
-Lemma eq_notauF_eq_eq_notauF': forall I (eutt : relation I) t s,
-  eq_notauF eutt t s <-> eq_notauF' eutt t s.
-Proof.
-  split; intros EUTT; destruct EUTT; eauto.
-  - econstructor; intros; subst; eauto.
-  - assert (u1 = u2) by (inv H; eauto).
-    subst. apply eq_dep_eq in H. subst. eauto.
-Qed.
-*)
-
-(* [eutt_ eutt t1 t2] means that, if [t1] or [t2] ever takes a
-   visible step ([Vis] or [Ret]), then the other takes the same
-   step, and the subsequent continuations (in the [Vis] case) are
-   related by [eutt]. In particular, [(t1 = spin)%eq_itree] if
-   and only if [(t2 = spin)%eq_itree]. Note also that in that
-   case, the parameter [eutt] is irrelevant.
-
-   This is the relation we will take a fixpoint of. *)
-Inductive euttF (eutt : itree E R1 -> itree E R2 -> Prop)
-          (ot1 : itreeF E R1 (itree E R1))
-          (ot2 : itreeF E R2 (itree E R2)) : Prop :=
-| euttF_ (FIN: finite_tausF ot1 <-> finite_tausF ot2)
-         (EQV: forall ot1' ot2'
-                  (UNTAUS1: unalltausF ot1 ot1')
-                  (UNTAUS2: unalltausF ot2 ot2'),
-               eq_notauF eutt ot1' ot2')
+Inductive euttF 
+              (eutt: itree E R1 -> itree E R2 -> Prop)
+              (eutt_taus: itreeF E R1 _ -> itreeF E R2 _ -> Prop)
+  : itreeF E R1 _ -> itreeF E R2 _ -> Prop :=
+| euttF_ret r1 r2
+      (RBASE: RR r1 r2):
+    euttF eutt eutt_taus (RetF r1) (RetF r2)
+| euttF_vis u (e : E u) k1 k2
+      (EUTTK: forall x, eutt (k1 x) (k2 x)):
+    euttF eutt eutt_taus (VisF e k1) (VisF e k2)
+| euttF_tau_tau t1 t2
+      (EQTAUS: eutt_taus (observe t1) (observe t2)):
+    euttF eutt eutt_taus (TauF t1) (TauF t2)
+| euttF_tau_left t1 ot2
+      (EQTAUS: euttF eutt eutt_taus (observe t1) ot2):
+    euttF eutt eutt_taus (TauF t1) ot2
+| euttF_tau_right ot1 t2
+      (EQTAUS: euttF eutt eutt_taus ot1 (observe t2)):
+    euttF eutt eutt_taus ot1 (TauF t2)
 .
 Hint Constructors euttF.
 
-Definition eutt_ (eutt : itree E R1 -> itree E R2 -> Prop)
-           (t1 : itree E R1) (t2 : itree E R2) : Prop :=
-  euttF eutt (observe t1) (observe t2).
+Definition eutt_ eutt t1 t2 := paco2 (euttF eutt) bot2 (observe t1) (observe t2).
 Hint Unfold eutt_.
 
-(* Paco takes the greatest fixpoints of monotone relations. *)
+Lemma euttF_mon r r' s s' x y
+    (EUTT: euttF r s x y)
+    (LEr: r <2= r')
+    (LEs: s <2= s'):
+  euttF r' s' x y.
+Proof.
+  induction EUTT; eauto.
+Qed.
 
-Lemma monotone_eq_notauF : forall I J (r r' : I -> J -> Prop) x1 x2
-      (IN: eq_notauF r x1 x2)
-      (LE: r <2= r'),
-    eq_notauF r' x1 x2.
-Proof. pmonauto. Qed.
-Hint Resolve monotone_eq_notauF.
+Lemma monotone_euttF eutt : monotone2 (euttF eutt).
+Proof. repeat intro. eauto using euttF_mon. Qed.
+Hint Resolve monotone_euttF : paco.
 
-(* [eutt_] is monotone. *)
 Lemma monotone_eutt_ : monotone2 eutt_.
-Proof. pmonauto. Qed.
+Proof. red. eauto using euttF_mon, paco2_mon_gen. Qed.
 Hint Resolve monotone_eutt_ : paco.
 
 (* We now take the greatest fixpoint of [eutt_]. *)
@@ -393,250 +88,61 @@ Hint Resolve monotone_eutt_ : paco.
 
    [eutt t1 t2]: [t1] is equivalent to [t2] up to taus. *)
 Definition eutt : itree E R1 -> itree E R2 -> Prop := paco2 eutt_ bot2.
+Hint Unfold eutt.
 
 Global Arguments eutt t1%itree t2%itree.
 
-Infix "≈" := eutt (at level 70) : itree_scope.
-
-(* Lemmas about the auxiliary relations. *)
-
-(* Many have a name [X_Y] to represent an implication
-   [X _ -> Y _] (possibly with more arguments on either side). *)
-
-(**)
-
-Lemma euttF_tau r t1 t2 t1' t2'
-    (OBS1: TauF t1' = observe t1)
-    (OBS2: TauF t2' = observe t2)
-    (REL: eutt_ r t1' t2'):
-  eutt_ r t1 t2.
-Proof.
-  intros. destruct REL. econstructor.
-  - simpobs. rewrite !finite_taus_tau. eauto.
-  - intros. eapply EQV; eapply unalltaus_tau; eauto.
-Qed.
-
-Lemma euttF_tau_left r t1 t2 t1'
-    (OBS: TauF t1 = observe t1')
-    (REL: eutt_ r t1' t2):
-  eutt_ r t1 t2.
-Proof.
-  intros. destruct REL. econstructor.
-  - rewrite <- FIN. symmetry. rewrite <- OBS. rewrite <- finite_taus_tau; eauto. reflexivity.
-  - intros. eapply EQV; eauto. rewrite <- OBS. inversion UNTAUS1. constructor; auto.
-    econstructor; eauto.
-Qed.
-
-Lemma euttF_tau_right r t1 t2 t2'
-    (OBS: TauF t2 = observe t2')
-    (REL: eutt_ r t1 t2'):
-  eutt_ r t1 t2.
-Proof.
-  intros. destruct REL. econstructor.
-  - rewrite FIN. rewrite <- OBS. rewrite <- finite_taus_tau; eauto. reflexivity.
-  - intros. eapply EQV; eauto. rewrite <- OBS. inversion UNTAUS2. constructor; auto.
-    econstructor; eauto.
-Qed.
-
-Lemma euttF_vis {u} (r : _ -> _ -> Prop) t1 t2 (e : _ u) k1 k2
-    (OBS1: VisF e k1 = observe t1)
-    (OBS2: VisF e k2 = observe t2)
-    (REL: forall x, r (k1 x) (k2 x)):
-  eutt_ r t1 t2.
-Proof.
-  intros. econstructor.
-  - split; intros; eapply notau_finite_taus; eauto.
-  - intros.
-    apply unalltaus_notau_id in UNTAUS1; eauto.
-    apply unalltaus_notau_id in UNTAUS2; eauto.
-    simpobs. subst. eauto.
-Qed.
-
-(**)
-
-Lemma eutt_strengthen :
-  forall r (t1 : itree E R1) (t2 : itree E R2)
-     (FIN: finite_taus t1 <-> finite_taus t2)
-     (EQV: forall t1' t2'
-              (UNT1: unalltaus t1 t1')
-              (UNT2: unalltaus t2 t2'),
-         paco2 (eutt_ ∘ gres2 eutt_) r t1' t2'),
-    paco2 (eutt_ ∘ gres2 eutt_) r t1 t2.
-Proof.
-  intros. pfold. econstructor; eauto.
-  intros.
-  hexploit (EQV (go ot1') (go ot2')); eauto.
-  intros EQV'. punfold EQV'. destruct EQV'.
-  eapply EQV0;
-    repeat constructor; eauto.
-Qed.
-
-(**)
-
-Lemma eq_unalltaus (t1 : itree E R1) (t2 : itree E R2) ot1'
-    (FT: unalltausF (observe t1) ot1')
-    (EQV: eq_itree RR t1 t2) :
-  exists ot2', unalltausF (observe t2) ot2'.
-Proof.
-  genobs t1 ot1. revert t1 Heqot1 t2 EQV.
-  destruct FT as [Huntaus Hnotau].
-  induction Huntaus; intros; punfold EQV; unfold_eq_itree; subst.
-  - eexists. constructor; eauto. inv EQV; simpl; eauto.
-  - inv EQV; simpobs; try inv Heqot1.
-    pclearbot. edestruct IHHuntaus as [? []]; eauto.
-Qed.
-
-Lemma eq_unalltaus_eqF (t : itree E R1) (s : itree E R2) ot'
-    (UNTAUS : unalltausF (observe t) ot')
-    (EQV: eq_itree RR t s) :
-  exists os', unalltausF (observe s) os' /\ eq_itreeF RR (eq_itree RR) ot' os'.
-Proof.
-  destruct UNTAUS as [Huntaus Hnotau].
-  remember (observe t) as ot. revert s t Heqot EQV.
-  induction Huntaus; intros; punfold EQV; unfold_eq_itree.
-  - eexists (observe s). split.
-    inv EQV; simpobs; eauto.
-    subst; eauto.
-    eapply eq_itreeF_mono; eauto.
-    intros ? ? [| []]; eauto.
-  - inv EQV; simpobs; inversion Heqot; subst.
-    destruct REL as [| []].
-    edestruct IHHuntaus as [? [[]]]; eauto 10.
-Qed.
-
-Lemma eq_unalltaus_eq (t : itree E R1) (s : itree E R2) t'
-    (UNTAUS : unalltausF (observe t) (observe t'))
-    (EQV: eq_itree RR t s) :
-  exists s', unalltausF (observe s) (observe s') /\ eq_itree RR t' s'.
-Proof.
-  eapply eq_unalltaus_eqF in UNTAUS; try eassumption.
-  destruct UNTAUS as [os' []]. eexists (go os'); split; eauto.
-  pfold. eapply eq_itreeF_mono; eauto.
-Qed.
-
-Lemma eutt_Ret x y :
-  RR x y -> eutt (Ret x) (Ret y).
-Proof.
-  intros; pfold.
-  constructor.
-  split; intros; eapply finite_taus_ret; reflexivity.
-  intros.
-  apply unalltausF_ret in UNTAUS1.
-  apply unalltausF_ret in UNTAUS2.
-  subst; constructor; assumption.
-Qed.
-
-Lemma eutt_Vis {U} (e: E U) k k' :
-  (forall x, eutt (k x) (k' x)) ->
-  eutt (Vis e k) (Vis e k').
-Proof.
-  intros.
-  pfold; constructor.
-  split; intros; eapply finite_taus_vis; reflexivity.
-  intros.
-  cbn in *.
-  apply unalltausF_vis in UNTAUS1.
-  apply unalltausF_vis in UNTAUS2.
-  subst; constructor.
-  intros x; specialize (H x).
-  punfold H.
-Qed.
-
 End EUTT.
 
-Hint Resolve monotone_eq_notauF.
-Hint Constructors eq_notauF.
 Hint Constructors euttF.
+Hint Unfold eutt_.
+Hint Resolve monotone_euttF : paco.
 Hint Resolve monotone_eutt_ : paco.
+Hint Unfold eutt.
 
-(** *** [eq_notauF] lemmas *)
+Infix "≈" := (eutt eq) (at level 70) : itree_scope.
 
-Lemma eq_notauF_and {E R1 R2} (RR : R1 -> R2 -> Prop) {I J}
-        (eutt1 eutt2 eutt : I -> J -> Prop) :
-  (forall t1 t2, eutt1 t1 t2 -> eutt2 t1 t2 -> eutt t1 t2) ->
-  forall (ot1 : itreeF E R1 I) (ot2 : itreeF E R2 J),
-    eq_notauF RR eutt1 ot1 ot2 -> eq_notauF RR eutt2 ot1 ot2 ->
-    eq_notauF RR eutt ot1 ot2.
+Section EUTT_homo.
+
+Context {E : Type -> Type} {R : Type} (RR : R -> R -> Prop).
+
+Global Instance subrelation_eq_eutt :
+  @subrelation (itree E R) (eq_itree RR) (eutt RR).
 Proof.
-  intros ? ? ? [] Hen2; inversion Hen2; auto.
-  auto_inj_pair2; subst; auto.
+  pcofix CIH. intros. pfold. revert_until CIH. pcofix CIH'. intros.
+  punfold H0. pfold. inv H0; pclearbot; eauto 7.
 Qed.
 
-Lemma eq_notauF_flip {E R1 R2} (RR : R1 -> R2 -> Prop) {I J}
-      (eutt : I -> J -> Prop) :
-  forall (ot1 : itreeF E R1 I) (ot2 : itreeF E R2 J),
-    eq_notauF (flip RR) (flip eutt) ot2 ot1 ->
-    eq_notauF RR eutt ot1 ot2.
+Global Instance Reflexive_eutt_gen `{Reflexive _ RR}
+       (r : itree E R -> itree E R -> Prop) :
+  Reflexive (paco2 (eutt_ RR) r).
 Proof.
-  intros ? ? []; auto.
+  pcofix CIH. intros. pfold. revert x. pcofix CIH'. intros.
+  genobs x ox. destruct ox; eauto.
 Qed.
 
-Delimit Scope eutt_scope with eutt.
-
-(** ** Generalized symmetry and transitivity *)
-
-Lemma Symmetric_eq_notauF_ {E R1 R2}
-      (RR1 : R1 -> R2 -> Prop) (RR2 : R2 -> R1 -> Prop)
-      {I J} (r1 : I -> J -> Prop) (r2 : J -> I -> Prop)
-      (SYM_RR : forall r1 r2, RR1 r1 r2 -> RR2 r2 r1)
-      (SYM_r : forall i j, r1 i j -> r2 j i)
-      (ot1 : itreeF E R1 I) (ot2 : itreeF E R2 J) :
-  eq_notauF RR1 r1 ot1 ot2 ->
-  eq_notauF RR2 r2 ot2 ot1.
-Proof. intros []; auto. Qed.
-
-Lemma Transitive_eq_notauF_ {E R1 R2 R3}
-      (RR1 : R1 -> R2 -> Prop) (RR2 : R2 -> R3 -> Prop)
-      (RR3 : R1 -> R3 -> Prop)
-      {I J K} (r1 : I -> J -> Prop) (r2 : J -> K -> Prop)
-      (r3 : I -> K -> Prop)
-      (TRANS_RR : forall r1 r2 r3, RR1 r1 r2 -> RR2 r2 r3 -> RR3 r1 r3)
-      (TRANS_r : forall i j k, r1 i j -> r2 j k -> r3 i k)
-      (ot1 : itreeF E R1 I) ot2 ot3 :
-  eq_notauF RR1 r1 ot1 ot2 ->
-  eq_notauF RR2 r2 ot2 ot3 ->
-  eq_notauF RR3 r3 ot1 ot3.
+Global Instance Reflexive_euttF_gen `{Reflexive _ RR}
+       (r : relation (itree E R)) (r' : relation (itree' E R)) :
+  Reflexive (euttF RR (upaco2 (eutt_ RR) r) (upaco2 (euttF RR (upaco2 (eutt_ RR) r)) r')). 
 Proof.
-  intros [] I2; inversion I2; eauto.
-  auto_inj_pair2; subst; eauto.
+  repeat intro. assert (X := Reflexive_eutt_gen r (go x)). do 2 punfold X.
+  eauto using euttF_mon, upaco2_mon_bot.
 Qed.
 
-Lemma Symmetric_euttF_ {E R1 R2}
-      (RR1 : R1 -> R2 -> Prop) (RR2 : R2 -> R1 -> Prop)
-      (r1 : _ -> _ -> Prop) (r2 : _ -> _ -> Prop)
-      (SYM_RR : forall r1 r2, RR1 r1 r2 -> RR2 r2 r1)
-      (SYM_r : forall i j, r1 i j -> r2 j i)
-      (ot1 : itree' E R1) (ot2 : itree' E R2) :
-  euttF RR1 r1 ot1 ot2 ->
-  euttF RR2 r2 ot2 ot1.
+Global Instance Symmetric_eutt_gen `{Symmetric _ RR}
+       (r : itree E R -> itree E R -> Prop)
+       (Sr : Symmetric r) :
+  Symmetric (paco2 (eutt_ RR) r).
 Proof.
-  intros []; split.
-  - split; apply FIN.
-  - intros. specialize (EQV _ _ UNTAUS2 UNTAUS1).
-    eapply Symmetric_eq_notauF_; eauto.
+  pcofix CIH. intros. pfold. revert_until CIH. pcofix CIH'. intros.
+  punfold H1. punfold H1. pfold.
+  genobs_clear x ox. genobs_clear y oy.
+  induction H1; pclearbot; eauto.
+  - econstructor. intros. destruct (EUTTK x); eauto.
+  - punfold EQTAUS. eauto 8.
 Qed.
 
-Lemma Transitive_euttF_ {E R1 R2 R3}
-      (RR1 : R1 -> R2 -> Prop) (RR2 : R2 -> R3 -> Prop)
-      (RR3 : R1 -> R3 -> Prop)
-      (r1 : _ -> _ -> Prop) (r2 : _ -> _ -> Prop)
-      (r3 : _ -> _ -> Prop)
-      (TRANS_RR : forall r1 r2 r3, RR1 r1 r2 -> RR2 r2 r3 -> RR3 r1 r3)
-      (TRANS_r : forall i j k, r1 i j -> r2 j k -> r3 i k)
-      (ot1 : itree' E R1) ot2 ot3 :
-  euttF RR1 r1 ot1 ot2 ->
-  euttF RR2 r2 ot2 ot3 ->
-  euttF RR3 r3 ot1 ot3.
-Proof.
-  intros [] [].
-  constructor.
-  - etransitivity; eauto.
-  - intros t1' t3' H1 H3.
-    assert (FIN2 : finite_tausF ot2).
-    { apply FIN; eauto. }
-    destruct FIN2 as [t2' []].
-    eapply Transitive_eq_notauF_; eauto.
-Qed.
+End EUTT_homo.
 
 Lemma Symmetric_eutt_ {E R1 R2}
       (RR1 : R1 -> R2 -> Prop) (RR2 : R2 -> R1 -> Prop)
@@ -646,206 +152,128 @@ Lemma Symmetric_eutt_ {E R1 R2}
   forall (t1 : itree E R1) (t2 : itree E R2),
     paco2 (eutt_ RR1) r1 t1 t2 -> paco2 (eutt_ RR2) r2 t2 t1.
 Proof.
-  pcofix self.
-  intros t1 t2 H12.
-  punfold H12.
-  pfold.
-  eapply Symmetric_euttF_; try eassumption.
-  intros ? ? []; auto.
-Qed.
-
-Lemma Transitive_eutt_ {E R1 R2 R3}
-      (RR1 : R1 -> R2 -> Prop) (RR2 : R2 -> R3 -> Prop)
-      (RR3 : R1 -> R3 -> Prop)
-      (TRANS_RR : forall r1 r2 r3, RR1 r1 r2 -> RR2 r2 r3 -> RR3 r1 r3) :
-  forall (t1 : itree E R1) t2 t3,
-    eutt RR1 t1 t2 -> eutt RR2 t2 t3 -> eutt RR3 t1 t3.
-Proof.
-  pcofix self.
-  intros t1 t2 t3 H12 H23.
-  punfold H12; punfold H23; pfold.
-  eapply Transitive_euttF_; try eassumption.
-  intros; pclearbot; eauto.
-Qed.
-
-Section EUTT_rel.
-
-Context {E : Type -> Type} {R : Type} (RR : R -> R -> Prop).
-
-(* Reflexivity of [eq_notauF], modulo a few assumptions. *)
-Lemma Reflexive_eq_notauF `{Reflexive _ RR} I (eq_ : I -> I -> Prop) :
-  Reflexive eq_ ->
-  forall (ot : itreeF E R I), notauF ot -> eq_notauF RR eq_ ot ot.
-Proof.
-  intros. destruct ot; try contradiction; econstructor; intros; subst; eauto.
-Qed.
-
-Global Instance Symmetric_eq_notauF `{Symmetric _ RR} I (eq_ : I -> I -> Prop) :
-  Symmetric eq_ -> Symmetric (@eq_notauF E _ _ RR _ _ eq_).
-Proof.
-  repeat intro. eapply Symmetric_eq_notauF_; eauto.
-Qed.
-
-Global Instance Transitive_eq_notauF `{Transitive _ RR} I (eq_ : I -> I -> Prop) :
-  Transitive eq_ -> Transitive (@eq_notauF E _ _ RR _ _ eq_).
-Proof.
-  repeat intro. eapply Transitive_eq_notauF_; eauto.
-Qed.
-
-Global Instance subrelation_eq_eutt :
-  @subrelation (itree E R) (eq_itree RR) (eutt RR).
-Proof.
   pcofix CIH. intros.
-  pfold. econstructor.
-  { split; [|apply flip_eq_itree in H0]; intros; destruct H as [n [? ?]]; eauto using eq_unalltaus. }
-
-  intros. eapply eq_unalltaus_eqF in H0; eauto. destruct H0 as [s' [UNTAUS' EQV']].
-  hexploit @unalltaus_injective; [apply UNTAUS' | apply UNTAUS2 | intro X]; subst.
-  inv EQV'; simpobs; eauto.
-  eapply unalltaus_notau in UNTAUS1. contradiction.
+  pfold. revert_until CIH. pcofix CIH'. intros.
+  pfold. do 2 punfold H0.
+  genobs_clear t1 ot1. genobs_clear t2 ot2.
+  induction H0; pclearbot; eauto 7.
+  econstructor; intros. edestruct EUTTK; eauto.
 Qed.
 
-Global Instance Reflexive_euttF `{Reflexive _ RR}
-       (r : itree E R -> itree E R -> Prop) :
-  Reflexive r -> Reflexive (euttF RR r).
+Section EUTT_eq_EUTTE.
+
+Context {E : Type -> Type} {R1 R2 : Type} (RR : R1 -> R2 -> Prop).
+
+Lemma euttE__impl_eutt_ r t1 t2 :
+  @euttE_ E R1 R2 RR r t1 t2 -> eutt_ RR r t1 t2.
 Proof.
-  split.
-  - reflexivity.
-  - intros.
-    erewrite (unalltaus_injective _ _ _ UNTAUS1 UNTAUS2).
-    apply Reflexive_eq_notauF; eauto.
+  revert t1 t2. pcofix CIH'. intros. destruct H0.
+  genobs t1 ot1. genobs t2 ot2. clear Heqot1 t1 Heqot2 t2.
+  assert (EM: notauF ot1 \/ notauF ot2 \/ ~(notauF ot1 \/ notauF ot2))
+    by (destruct ot1, ot2; simpl; tauto).
+  destruct EM as [EM|[EM|EM]].
+  - destruct FIN as [FIN _].
+    hexploit FIN; eauto 7. clear FIN; intro FIN.
+    destruct FIN as [ot' [UNTAUS NOTAU]].
+    hexploit EQV; eauto. intros EQNT.
+    induction UNTAUS; subst.
+    { pfold. inv EQNT; eauto. }
+    hexploit IHUNTAUS; eauto.
+    { intros. destruct UNTAUS1.
+      dependent destruction H; [|subst; contradiction].
+      hexploit @unalltaus_injective; [|econstructor|]; eauto. intros; subst; eauto.
+    }
+    intros EUTT. punfold EUTT.
+  - destruct FIN as [_ FIN].
+    hexploit FIN; eauto 7. clear FIN; intro FIN.
+    destruct FIN as [ot' [UNTAUS NOTAU]].
+    hexploit EQV; eauto. intros EQNT.
+    induction UNTAUS; subst.
+    { pfold. inv EQNT; eauto. }
+    hexploit IHUNTAUS; eauto.
+    { intros. destruct UNTAUS2.
+      dependent destruction H; [|subst; contradiction].
+      hexploit @unalltaus_injective; [|econstructor|]; eauto. intros; subst; eauto.
+    }
+    intros EUTT. punfold EUTT.
+  - destruct ot1, ot2; simpl in *; try tauto.
+    pfold. econstructor. right. apply CIH'.
+    econstructor.
+    + rewrite !finite_taus_tau in FIN. eauto.
+    + eauto using unalltaus_tau'.
 Qed.
 
-Global Instance Symmetric_euttF `{Symmetric _ RR}
-         (r : itree E R -> itree E R -> Prop) :
-  Symmetric r -> Symmetric (euttF RR r).
+Lemma eutt__impl_euttE_ r t1 t2 :
+  @eutt_ E R1 R2 RR r t1 t2 -> euttE_ RR r t1 t2.
 Proof.
-  intros SYM x y. apply Symmetric_euttF_; auto.
+  intros. punfold H. econstructor; intros.
+  - split; intros.
+    + genobs t1 ot1. genobs t2 ot2. clear Heqot1 t1 Heqot2 t2.
+      destruct H0 as [ot' [UNTAUS NOTAU]].
+      move UNTAUS before r. revert_until UNTAUS.
+      induction UNTAUS; intros.
+      * induction H; eauto; try contradiction.
+        rewrite finite_taus_tau. eauto.
+      * induction H; eauto 7; try inv OBS; pclearbot
+        ; rewrite ?finite_taus_tau; eauto; eapply IHUNTAUS; eauto.
+        punfold EQTAUS.
+   + genobs t1 ot1. genobs t2 ot2. clear Heqot1 t1 Heqot2 t2.
+     destruct H0 as [ot' [UNTAUS NOTAU]].
+     move UNTAUS before r. revert_until UNTAUS.
+     induction UNTAUS; intros.
+     * induction H; eauto; try contradiction.
+       rewrite finite_taus_tau. eauto.
+     * induction H; eauto 7; try inv OBS; pclearbot
+       ; rewrite ?finite_taus_tau; eauto; eapply IHUNTAUS; eauto.
+       punfold EQTAUS.
+  - genobs t1 ot1. genobs t2 ot2. clear Heqot1 t1 Heqot2 t2.
+    destruct UNTAUS1 as [UNTAUS1 NT1]. destruct UNTAUS2 as [UNTAUS2 NT2].
+    move UNTAUS2 before r. move UNTAUS1 before r. revert_until UNTAUS1.
+    induction UNTAUS1.
+    + induction 1; intros.
+      * inv H; try contradiction; eauto.
+      * subst. inv H; try contradiction. eauto.
+    + induction 1; intros; subst.
+      * inv H; try contradiction; eauto.
+      * inv H; try contradiction; eauto.
+        pclearbot. eapply IHUNTAUS1; eauto.
+        punfold EQTAUS.
 Qed.
 
-Global Instance Transitive_euttF `{Transitive _ RR}
-       (r : itree E R -> itree E R -> Prop) :
-  Transitive r -> Transitive (euttF RR r).
+Lemma eutt__is_euttE_ r t1 t2 :
+  @eutt_ E R1 R2 RR r t1 t2 <-> euttE_ RR r t1 t2.
+Proof. split; eauto using euttE__impl_eutt_, eutt__impl_euttE_. Qed.
+
+Lemma euttE_impl_eutt r t1 t2 :
+  paco2 (@euttE_ E R1 R2 RR) r t1 t2 -> paco2 (eutt_ RR) r t1 t2.
 Proof.
-  intros TRANS x y z. apply Transitive_euttF_; auto.
+  split; intros; eapply paco2_mon_gen; eauto; intros; apply euttE__impl_eutt_; eauto.
 Qed.
 
-Global Instance Symmetric_eutt `{Symmetric _ RR}
-       (r : itree E R -> itree E R -> Prop)
-       (Sr : Symmetric r) :
-  Symmetric (paco2 (eutt_ RR) r).
-Proof. red; eapply Symmetric_eutt_; eauto. Qed.
-
-Global Instance Reflexive_eutt `{Reflexive _ RR}
-       (r : itree E R -> itree E R -> Prop) :
-  Reflexive (paco2 (eutt_ RR) r).
+Lemma eutt_impl_euttE r t1 t2 :
+  paco2 (@eutt_ E R1 R2 RR) r t1 t2 -> paco2 (euttE_ RR) r t1 t2.
 Proof.
-  pcofix CIH.
-  intros. pfold. red. apply Reflexive_euttF; eauto.
+  split; intros; eapply paco2_mon_gen; eauto; intros; apply eutt__impl_euttE_; eauto.
 Qed.
 
-End EUTT_rel.
+Lemma eutt_is_euttE r t1 t2 :
+  paco2 (@eutt_ E R1 R2 RR) r t1 t2 <-> paco2 (euttE_ RR) r t1 t2.
+Proof. split; eauto using euttE_impl_eutt, eutt_impl_euttE. Qed.
 
-Section EUTT_eq.
+End EUTT_eq_EUTTE.
 
-Context {E : Type -> Type} {R : Type}.
+Section EUTT_trans.
 
-Let eutt : itree E R -> itree E R -> Prop := eutt eq.
+Context {E : Type -> Type} {R1 R2 : Type} (RR : R1 -> R2 -> Prop).
 
-Infix "≈" := eutt (at level 70) : itree_scope.
+Ltac convert_eutt_to_euttE :=
+  try (apply euttE__impl_eutt_ || apply euttE_impl_eutt);
+  repeat match goal with [H: eutt_ _ _ _ _ |- _] => apply eutt__impl_euttE_ in H end;
+  repeat match goal with [H: eutt _ _ _ |- _] => apply eutt_impl_euttE in H end.
 
-Global Instance Transitive_eutt : Transitive eutt.
-Proof.
-  red; eapply Transitive_eutt_; eauto.
-  intros; subst; eauto.
-Qed.
-
-(**)
-
-(* [eutt] is preserved by removing one [Tau]. *)
-Lemma tauF_eutt (t t': itree E R) (OBS: TauF t' = observe t): t ≈ t'.
-Proof.
-  pfold. split.
-  - simpobs. rewrite finite_taus_tau. reflexivity.
-  - intros t1' t2' H1 H2.
-    eapply unalltaus_tau in H1; eauto.
-    pose proof (unalltaus_injective _ _ _ H1 H2).
-    subst; apply Reflexive_eq_notauF; eauto.
-    left. apply reflexivity.
-Qed.
-
-Lemma tau_eutt (t: itree E R) : Tau t ≈ t.
-Proof.
-  eapply tauF_eutt. eauto.
-Qed.
-
-(* [eutt] is preserved by removing all [Tau]. *)
-Lemma untaus_eutt (t t' : itree E R) : untausF (observe t) (observe t') -> t ≈ t'.
-Proof.
-  intros H.
-  pfold. split.
-  - eapply untaus_finite_taus; eauto.
-  - induction H; intros.
-    + rewrite (unalltaus_injective _ _ _ UNTAUS1 UNTAUS2).
-      apply Reflexive_eq_notauF; eauto.
-      left; apply reflexivity.
-    + eapply unalltaus_tau in UNTAUS1; eauto.
-Qed.
-
-(* We can now rewrite with [eutt] equalities. *)
-Global Instance Equivalence_eutt : @Equivalence (itree E R) eutt.
-Proof. constructor; typeclasses eauto. Qed.
-
-(**)
-
-Global Instance eutt_go : Proper (going eutt ==> eutt) go.
-Proof. intros ? ? []; eauto. Qed.
-
-Global Instance eutt_observe : Proper (eutt ==> going eutt) observe.
-Proof.
-  constructor. punfold H. pfold. destruct H. econstructor; eauto.
-Qed.
-
-Global Instance eutt_tauF : Proper (eutt ==> going eutt) (fun t => TauF t).
-Proof.
-  constructor; pfold. punfold H.
-  destruct H. econstructor.
-  - split; intros; simpl.
-    + rewrite finite_taus_tau, <-FIN, <-finite_taus_tau; eauto.
-    + rewrite finite_taus_tau, FIN, <-finite_taus_tau; eauto.
-  - intros. eapply EQV; eapply unalltaus_tau; eauto.
-Qed.
-
-Global Instance eutt_VisF {u} (e: E u) :
-  Proper (pointwise_relation _ eutt ==> going eutt) (VisF e).
-Proof.
-  constructor; pfold. red in H. econstructor.
-  - repeat econstructor.
-  - intros.
-    destruct UNTAUS1 as [UNTAUS1 Hnotau1].
-    destruct UNTAUS2 as [UNTAUS2 Hnotau2].
-    dependent destruction UNTAUS1.
-    dependent destruction UNTAUS2. simpobs.
-    econstructor; intros; left; apply H.
-Qed.
-
-Global Instance eq_itree_notauF :
-  Proper (going (@eq_itree E R _ eq) ==> flip impl) notauF.
-Proof.
-  intros ? ? [] ?; punfold H. inv H; simpl in *; subst; eauto.
-Qed.
-
-(* If [t1] and [t2] are equivalent, then either both start with
-   finitely many taus, or both [spin]. *)
-Global Instance eutt_finite_taus :
-  Proper (going eutt ==> flip impl) finite_tausF.
-Proof.
-  intros ? ? [] ?; punfold H. eapply H. eauto.
-Qed.
-
-Inductive eutt_trans_clo (r: itree E R -> itree E R -> Prop) :
-  itree E R -> itree E R -> Prop :=
-| eutt_pre_clo_intro (t1 t2 t3 t4: itree E R)
+Inductive eutt_trans_clo (r: itree E R1 -> itree E R2 -> Prop) :
+  itree E R1 -> itree E R2 -> Prop :=
+| eutt_pre_clo_intro t1 t2 t3 t4
       (EQVl: t1 ≈ t2)
       (EQVr: t4 ≈ t3)
       (REL: r t2 t3)
@@ -853,38 +281,147 @@ Inductive eutt_trans_clo (r: itree E R -> itree E R -> Prop) :
 .
 Hint Constructors eutt_trans_clo.
 
-Lemma eutt_clo_trans : weak_respectful2 (eutt_ eq) eutt_trans_clo.
+Lemma eutt_clo_trans :
+  weak_respectful2 (@eutt_ E R1 R2 RR) eutt_trans_clo.
 Proof.
   econstructor; [pmonauto|].
-  intros. inv PR.
-  punfold EQVl. punfold EQVr. destruct EQVl, EQVr. split.
-  { rewrite FIN, FIN0. apply GF in REL. destruct REL. eauto. }
+  intros. destruct PR.
+  convert_eutt_to_euttE.
+  destruct (euttE_clo_trans E _ _ RR). clear WEAK_MON.
+  hexploit WEAK_RESPECTFUL.
+  { apply LE. }
+  { intros. apply GF in PR. convert_eutt_to_euttE. auto. }
+  { econstructor; [apply EQVl|apply EQVr|apply REL]. }
+  intros EUTT.
+  eapply monotone_euttE_; eauto; intros.
+  eapply rclo2_mon_gen; eauto; intros.
+  - convert_eutt_to_euttE. auto.
+  - destruct PR0. econstructor; convert_eutt_to_euttE; eauto.
+Qed.
 
-  intros. apply proj1 in FIN. edestruct FIN as [n'' [t2'' TAUS'']]; [eexists; eauto|].
-  hexploit EQV; eauto. intros EUTT1.
-  apply proj1 in FIN0. edestruct FIN0 as [n''' [t2''' TAUS''']]; [eexists; eauto|].
-  hexploit EQV0; eauto. intros EUTT2.
-  apply GF in REL. destruct REL.
-  hexploit EQV1; eauto. intros EUTT3.
-  destruct EUTT1; destruct EUTT2;
-    try (solve [subst; inversion EUTT3; auto]).
-  remember (VisF _ _) as o2 in EUTT3.
-  remember (VisF _ _) as o3 in EUTT3.
-  inversion EUTT3; subst; try discriminate.
-  inversion H2; clear H2; inversion H3; clear H3.
-  subst; auto_inj_pair2; subst.
-  econstructor. intros.
-  specialize (H x); specialize (H0 x); specialize (H1 x).
-  pclearbot. eauto using rclo2.
+Global Instance eutt_cong_eutt r :
+  Proper (eutt eq ==> eutt eq ==> flip impl)
+         (paco2 (@eutt_ E R1 R2 RR ∘ gres2 (eutt_ RR)) r).
+Proof.
+  repeat intro. pupto2 eutt_clo_trans. eauto.
+Qed.
+
+Global Instance eutt_cong_gres_eutt_ r :
+  Proper (eutt eq ==> eutt eq ==> flip impl)
+         (gres2 (@eutt_ E R1 R2 RR) r).
+Proof.
+  repeat intro. pupto2 eutt_clo_trans. eauto.
+Qed.
+
+Global Instance eutt_eq_under_rr_impl :
+  Proper (@eutt E _ _ eq ==> @eutt _ _ _ eq ==> flip impl) (eutt RR).
+Proof.
+  repeat red. intros. pupto2_init. rewrite H, H0. pupto2_final. eauto.
+Qed.
+
+End EUTT_trans.
+
+Arguments eutt_clo_trans : clear implicits.
+Hint Constructors eutt_trans_clo.
+
+Section EUTT_nested_trans.
+
+Context {E : Type -> Type} {R1 R2 : Type} (RR : R1 -> R2 -> Prop).
+
+Inductive eutt_nested_trans_clo (r: itree' E R1 -> itree' E R2 -> Prop) :
+  itree' E R1 -> itree' E R2 -> Prop :=
+| eutt_nested_pre_clo_intro ot1 ot2 ot3 ot4
+      (EQVl: go ot1 ≅ go ot2)
+      (EQVr: go ot4 ≅ go ot3)
+      (REL: r ot2 ot3)
+  : eutt_nested_trans_clo r ot1 ot4
+.
+Hint Constructors eutt_nested_trans_clo.
+
+Lemma eutt_nested_clo_trans r :
+  weak_respectful2 (euttF RR (gres2 (eutt_ RR) (upaco2 (eutt_ RR ∘ gres2 (eutt_ RR)) r)))
+                    eutt_nested_trans_clo.
+Proof.
+  econstructor; [pmonauto|].
+  intros. destruct PR.
+  apply GF in REL. clear l LE GF.
+  punfold EQVl; red in EQVl. punfold EQVr; red in EQVr. simpl in *.
+  move REL before r0. revert_until REL.
+  induction REL; intros; subst;
+    try (dependent destruction EQVl; dependent destruction EQVr; [ idtac ]; pclearbot).
+  - eauto.
+  - econstructor. intros. rewrite REL, REL0. eauto.
+  - econstructor. eapply rclo2_step. econstructor.
+    + rewrite REL. reflexivity.
+    + rewrite REL0. reflexivity.
+    + eauto using rclo2.
+  - dependent destruction EQVl; pclearbot. punfold REL0.
+  - dependent destruction EQVr; pclearbot. punfold REL0.
+Qed.
+
+Global Instance eq_cong_nested_euttF r r0 :
+  Proper (going (eq_itree eq) ==> going (eq_itree eq) ==> flip impl)
+         (paco2 (@euttF E R1 R2 RR (gres2 (eutt_ RR) (upaco2 (eutt_ RR ∘ gres2 (eutt_ RR)) r))
+                 ∘ gres2 (euttF RR (gres2 (eutt_ RR) (upaco2 (eutt_ RR ∘ gres2 (eutt_ RR)) r)))) r0).
+Proof.
+  repeat intro. destruct H, H0.
+  pupto2 eutt_nested_clo_trans. econstructor; eauto.
+Qed.
+
+End EUTT_nested_trans.
+
+Arguments eutt_nested_clo_trans : clear implicits.
+Hint Constructors eutt_nested_trans_clo.
+
+Section EUTT_eq.
+
+Context {E : Type -> Type} {R : Type}.
+
+Let eutt : itree E R -> itree E R -> Prop := eutt eq.
+
+Global Instance subrelation_observing_eutt:
+  @subrelation (itree E R) (observing eq) eutt.
+Proof.
+  repeat intro. eapply subrelation_eq_eutt, observing_eq_itree_eq. eauto.
+Qed.
+
+Global Instance Reflexive_eutt: Reflexive eutt.
+Proof. apply Reflexive_eutt_gen; eauto. Qed.
+
+Global Instance Symmetric_eutt: Symmetric eutt.
+Proof. apply Symmetric_eutt_gen; eauto. Qed.
+
+Global Instance Transitive_eutt : Transitive eutt.
+Proof.
+  unfold eutt. repeat intro. pupto2_init.
+  rewrite H, H0. pupto2_final. apply Reflexive_eutt.
+Qed.
+
+(* We can now rewrite with [eutt] equalities. *)
+Global Instance Equivalence_eutt : @Equivalence (itree E R) eutt.
+Proof. constructor; typeclasses eauto. Qed.
+
+Global Instance eutt_cong_go : Proper (going eutt ==> eutt) go.
+Proof. intros ? ? []; eauto. Qed.
+
+Global Instance eutt_cong_observe : Proper (eutt ==> going eutt) observe.
+Proof.
+  constructor. punfold H. pfold. destruct H. econstructor; eauto.
+Qed.
+
+Global Instance eutt_cong_tauF : Proper (eutt ==> going eutt) (@TauF _ _ _).
+Proof.
+  constructor. pfold. pfold. econstructor. punfold H.
+Qed.
+
+Global Instance eutt_cong_VisF {u} (e: E u) :
+  Proper (pointwise_relation _ eutt ==> going eutt) (VisF e).
+Proof. 
+  constructor. pfold. pfold. econstructor.
+  intros. specialize (H x0). punfold H.
 Qed.
 
 End EUTT_eq.
-
-Arguments eutt_clo_trans : clear implicits.
-
-Hint Constructors eutt_trans_clo.
-
-Infix "≈" := (eutt eq) (at level 70) : itree_scope.
 
 (**)
 
@@ -892,170 +429,74 @@ Lemma eutt_tau {E R1 R2} (RR : R1 -> R2 -> Prop)
            (t1 : itree E R1) (t2 : itree E R2) :
   eutt RR t1 t2 -> eutt RR (Tau t1) (Tau t2).
 Proof.
-  intros H.
-  pfold. eapply euttF_tau. reflexivity. reflexivity. punfold H.
+  intros. pfold. pfold. econstructor. punfold H.
 Qed.
 
-Lemma eq_itree_vis {E R1 R2} (RR : R1 -> R2 -> Prop)
+Lemma eutt_vis {E R1 R2} (RR : R1 -> R2 -> Prop)
       {U} (e : E U) (k1 : U -> itree E R1) (k2 : U -> itree E R2) :
-  (forall u, eq_itree RR (k1 u) (k2 u)) ->
-  eq_itree RR (Vis e k1) (Vis e k2).
+  (forall u, eutt RR (k1 u) (k2 u)) ->
+  eutt RR (Vis e k1) (Vis e k2).
 Proof.
-  intros; pfold; constructor; left. apply H.
+  intros. pfold. pfold. econstructor. intros. specialize (H x). punfold H.
 Qed.
 
-Lemma eq_itree_ret {E R1 R2} (RR : R1 -> R2 -> Prop) r1 r2 :
-  RR r1 r2 -> @eq_itree E _ _ RR (Ret r1) (Ret r2).
+Lemma eutt_ret {E R1 R2} (RR : R1 -> R2 -> Prop) r1 r2 :
+  RR r1 r2 -> @eutt E R1 R2 RR (Ret r1) (Ret r2).
 Proof.
-  intros; pfold; eauto; constructor; auto.
+  intros. pfold. pfold. econstructor. eauto.
 Qed.
 
-(* Lemmas about [bind]. *)
-
-Lemma untaus_bind {E S R} : forall t t' (k: S -> itree E R)
-      (UNTAUS: untausF (observe t) (observe t')),
-  untausF (observe (ITree.bind t k)) (observe (ITree.bind t' k)).
-Proof.
-  intros. genobs t ot; genobs t' ot'. revert t Heqot t' Heqot'.
-  induction UNTAUS; intros; subst.
-  - rewrite !unfold_bind; simpobs; eauto.
-  - rewrite unfold_bind. simpobs. cbn. eauto.
-Qed.
-
-Lemma untaus_bindF {E S R} : forall t t' (k: S -> itree E R)
-      (UNTAUS: untausF (observe t) t'),
-  untausF (observe (ITree.bind t k)) (observe (ITree.bind (go t') k)).
-Proof.
-  intros; eapply untaus_bind; eauto.
-Qed.
-
-Lemma finite_taus_bind_fst {E R S}
-      (t : itree E R) (f : R -> itree E S) :
-  finite_taus (ITree.bind t f) -> finite_taus t.
-Proof.
-  intros [tf' [TAUS PROP]].
-  genobs (ITree.bind t f) obtf. move TAUS at top. revert_until TAUS.
-  induction TAUS; intros; subst.
-  - rewrite unfold_bind in PROP.
-    genobs t ot; destruct ot; eauto using finite_taus_ret, finite_taus_vis.
-  - genobs t ot; destruct ot; eauto using finite_taus_ret, finite_taus_vis.
-    rewrite unfold_bind in Heqobtf. simpobs. inv Heqobtf. unfold_bind.
-    eapply finite_taus_tau; eauto.
-Qed.
-
-Lemma finite_taus_bind {E R S}
-      (t : itree E R) (f : R -> itree E S)
-      (FINt: finite_tausF (observe t))
-      (FINk: forall v, finite_tausF (observe (f v))):
-  finite_tausF (observe (ITree.bind t f)).
-Proof.
-  rewrite unfold_bind.
-  genobs t ot. clear Heqot t.
-  destruct FINt as [ot' [UNT NOTAU]].
-  induction UNT; subst.
-  - destruct ot0; inv NOTAU; simpl; eauto 7.
-  - apply finite_taus_tau. eauto.
-Qed.
-
-Inductive eutt_bind_clo {E R} (r: relation (itree E R)) : relation (itree E R) :=
-| eutt_bind_clo_intro U (t1 t2: itree E U) k1 k2
-      (EQV: t1 ≈ t2)
-      (REL: forall v, r (k1 v) (k2 v))
-  : eutt_bind_clo r (ITree.bind t1 k1) (ITree.bind t2 k2)
-.
-Hint Constructors eutt_bind_clo.
-
-Lemma bind_clo_finite_taus E U R (t1 t2: itree E U) (k1 k2: U -> itree E R)
-    (FT: finite_taus (ITree.bind t1 k1))
-    (FTk: forall v, finite_taus (k1 v) -> finite_taus (k2 v))
-    (EQV: t1 ≈ t2):
-  finite_taus (ITree.bind t2 k2).
-Proof.
-  punfold EQV. destruct EQV as [[FTt _] EQV].
-  assert (FT1 := FT). apply finite_taus_bind_fst in FT1.
-  assert (FT2 := FT1). apply FTt in FT2.
-  destruct FT1 as [a [FT1 NT1]], FT2 as [b [FT2 NT2]].
-  rewrite @untaus_finite_taus in FT; [|eapply untaus_bindF, FT1].
-  rewrite unfold_bind. genobs t2 ot2. clear Heqot2 t2.
-  induction FT2.
-  - destruct ot0; inv NT2; simpl; eauto 7.
-    hexploit EQV; eauto. intros EQV'. inv EQV'.
-    rewrite unfold_bind in FT. eauto.
-  - subst. eapply finite_taus_tau; eauto.
-    eapply IHFT2; eauto using unalltaus_tau'.
-Qed.
-
-Lemma eutt_clo_bind E R: weak_respectful2 (@eutt_ E R _ eq) eutt_bind_clo.
-Proof.
-  econstructor; [pmonauto|].
-  intros. destruct PR. split.
-  - assert (EQV':=EQV). symmetry in EQV'.
-    split; intros; eapply bind_clo_finite_taus; eauto; intros.
-    + edestruct GF; eauto. apply FIN. eauto.
-    + edestruct GF; eauto. apply FIN. eauto.
-  - punfold EQV. destruct EQV.
-    intros.
-    hexploit (@finite_taus_bind_fst E); [do 2 eexists; apply UNTAUS1|]. intros [a FT1].
-    hexploit (@finite_taus_bind_fst E); [do 2 eexists; apply UNTAUS2|]. intros [b FT2].
-    specialize (EQV _ _ FT1 FT2).
-    destruct FT1 as [FT1 Hnotau1]. destruct FT2 as [FT2 Hnotau2].
-    hexploit @untaus_bindF; [ eapply FT1 | ]. intros UT1.
-    hexploit @untaus_bindF; [ eapply FT2 | ]. intros UT2.
-    hexploit @untaus_unalltaus_rev; [apply UT1| |]. eauto. intros UAT1.
-    hexploit @untaus_unalltaus_rev; [apply UT2| |]; eauto. intros UAT2.
-    inv EQV.
-    + rewrite unfold_bind in UAT1, UAT2. simpobs. cbn in *.
-      eapply GF in REL. destruct REL.
-      eapply monotone_eq_notauF; eauto using rclo2.
-    + rewrite unfold_bind in UAT1, UAT2. simpobs. cbn in *.
-      destruct UAT1 as [UAT1 _]. destruct UAT2 as [UAT2 _].
-      dependent destruction UAT1. dependent destruction UAT2. simpobs.
-      econstructor. intros. specialize (H x). pclearbot. fold_bind. eauto using rclo2.
-Qed.
-
-(* [eutt] is a congruence wrt. [bind] *)
-
-Global Instance eutt_bind {E R S} :
+Global Instance eutt_bind {E S R} :
   Proper (eutt eq ==>
           pointwise_relation _ (eutt eq) ==>
           eutt eq) (@ITree.bind E R S).
 Proof.
-  repeat intro. pupto2_init.
-  pupto2 eutt_clo_bind. econstructor; eauto.
-  intros. pupto2_final. apply H0.
-Qed.
-
-Global Instance eutt_paco {E R} r:
-  Proper (eutt eq ==> eutt eq ==> flip impl)
-         (paco2 (@eutt_ E R _ eq ∘ gres2 (eutt_ eq)) r).
-Proof.
-  repeat intro. pupto2 eutt_clo_trans. eauto.
-Qed.
-
-Global Instance eutt_gres {E R} r:
-  Proper (eutt eq ==> eutt eq ==> flip impl)
-         (gres2 (@eutt_ E R _ eq) r).
-Proof.
-  repeat intro. pupto2 eutt_clo_trans. eauto.
+  repeat intro. do 2 punfold H.
+  revert_until S. pcofix CIH. intros.
+  pfold. revert_until CIH. pcofix CIH'. intros. pfold.
+  rewrite !unfold_bind. genobs_clear x ox. genobs_clear y oy.
+  move H0 before CIH'. revert_until H0.
+  induction H0; intros; subst; pclearbot.
+  - simpl. specialize (H1 r2). do 2 punfold H1.
+    eauto 7 using euttF_mon, upaco2_mon_bot.
+  - econstructor. intros.
+    specialize (EUTTK x). do 2 punfold EUTTK.
+  - econstructor. intros. punfold EQTAUS.
+  - econstructor. rewrite unfold_bind. eauto.
+  - econstructor. rewrite unfold_bind. eauto.
 Qed.
 
 Global Instance eutt_map {E R S} :
   Proper (pointwise_relation _ eq ==> eutt eq ==> eutt eq) (@ITree.map E R S).
 Proof.
-  unfold ITree.map. repeat red.
-  intros; eapply eutt_bind; eauto.
-  intro. rewrite H. reflexivity.
+  unfold ITree.map. do 3 red. intros.
+  rewrite H0. setoid_rewrite H. reflexivity.
 Qed.
 
 Global Instance eutt_forever {E R S} :
   Proper (eutt eq ==> eutt eq) (@ITree.forever E R S).
 Proof.
-Admitted.
+  cut (forall X (t1 t2: itree E X) (x y: itree E R), t1 ≈ t2 -> x ≈ y -> (t1 ;; @ITree.forever E R S x) ≈ (t2 ;; ITree.forever y)).
+  { repeat intro.
+    rewrite <-(ret_bind tt (fun _ => ITree.forever x)).
+    rewrite <-(ret_bind tt (fun _ => ITree.forever y)).
+    eapply H; eauto; reflexivity.
+  }
+
+  pcofix CIH. intros. 
+  pfold. revert_until CIH. pcofix CIH'. intros.
+  do 2 punfold H0. pfold.
+  rewrite !unfold_bind. genobs_clear t1 ot1. genobs_clear t2 ot2.
+  induction H0; intros; subst; pclearbot; try (econstructor; eauto 7; fail).
+  simpl. rewrite (unfold_forever x), (unfold_forever y). 
+  econstructor. eauto 7.
+Qed.
 
 Global Instance eutt_when {E} (b : bool) :
   Proper (eutt eq ==> eutt eq) (@ITree.when E b).
 Proof.
-Admitted.
+  repeat intro. destruct b; simpl; eauto. reflexivity.
+Qed.
 
 Lemma eutt_map_map {E R S T}
       (f : R -> S) (g : S -> T) (t : itree E R) :
@@ -1065,207 +506,7 @@ Proof.
   apply subrelation_eq_eutt, map_map.
 Qed.
 
-Lemma eutt_eq_under_rr_impl {E : Type -> Type}
-       {R1 R2 : Type} (RR: R1 -> R2 -> Prop):
-  Proper (@eutt E _ _ eq ==> @eutt _ _ _ eq ==> impl) (eutt RR).
+Lemma tau_eutt {E R} (t: itree E R) : Tau t ≈ t.
 Proof.
-  repeat intro.
-  symmetry in H.
-  eapply Transitive_eutt_; try eassumption.
-  2: eapply Transitive_eutt_; try eassumption.
-  all: intros; subst; eauto.
-Qed.
-
-Global Instance eutt_eq_under_rr {E : Type -> Type}
-       {R1 R2 : Type} (RR: R1 -> R2 -> Prop):
-  Proper (@eutt E _ _ eq ==> @eutt _ _ _ eq ==> iff) (eutt RR).
-Proof.
-  repeat intro.
-  split; eapply eutt_eq_under_rr_impl; auto.
-  all: symmetry; auto.
-Qed.
-
-Inductive euttF1' {E R} (r : itree E R -> itree E R -> Prop) :
-  itree' E R -> itree' E R -> Prop :=
-| euttF1_Tau_L : forall t1 t2,
-    euttF1' r t1.(observe) t2 ->
-    euttF1' r (TauF t1) t2
-| euttF1_Tau_R : forall t1 t2,
-    euttF1' r t1 t2.(observe) ->
-    euttF1' r t1 (TauF t2)
-| euttF1_euttF0 : forall t1 t2,
-    eq_notauF eq r t1 t2 ->
-    euttF1' r t1 t2
-.
-
-Definition euttF1 {E R} (r : relation (itree E R)) :
-  relation (itree E R) := observing (euttF1' r).
-
-Lemma euttF1_euttF {E R} (r : relation (itree E R)) :
-  forall t1 t2,
-    euttF1 r t1 t2 -> eutt_ eq r t1 t2.
-Proof.
-Admitted.
-
-Inductive euttF' {E R} (eutt: relation (itree E R)) (eqtaus: relation (itreeF E R _))
-  : relation (itreeF E R _) :=
-| euttF'_ret r : euttF' eutt eqtaus (RetF r) (RetF r)
-| euttF'_vis u (e : E u) k1 k2
-      (EUTTK: forall x, eutt (k1 x) (k2 x)):
-    euttF' eutt eqtaus (VisF e k1) (VisF e k2)
-| euttF'_tau_tau t1 t2
-      (EQTAUS: eqtaus (observe t1) (observe t2)):
-    euttF' eutt eqtaus (TauF t1) (TauF t2)
-| euttF'_tau_left t1 ot2
-      (EQTAUS: euttF' eutt eqtaus (observe t1) ot2):
-    euttF' eutt eqtaus (TauF t1) ot2
-| euttF'_right ot1 t2
-      (EQTAUS: euttF' eutt eqtaus ot1 (observe t2)):
-    euttF' eutt eqtaus ot1 (TauF t2)
-.
-Hint Constructors euttF'.
-
-Definition eutt'_ {E R} eutt t1 t2 := paco2 (@euttF' E R eutt) bot2 (* (fun x y => eutt (go x) (go y)) *) (observe t1) (observe t2).
-Hint Unfold eutt'_.
-
-Definition eutt' {E R} := paco2 (@eutt'_ E R) bot2.
-Hint Unfold eutt'.
-
-Lemma euttF'_mon {E R} r r' s s' x y
-    (EUTT: @euttF' E R r s x y)
-    (LEr: r <2= r')
-    (LEs: s <2= s'):
-  euttF' r' s' x y.
-Proof.
-  induction EUTT; eauto.
-Qed.
-
-Lemma reflexive_euttF' {E R} eutt eqtaus (r1:Reflexive eutt) (r:Reflexive eqtaus) : Reflexive (@euttF' E R eutt eqtaus).
-Proof.
-  unfold Reflexive. intros x.
-  destruct x; eauto.
-Qed.
-
-Lemma monotone_euttF' {E R} eutt : monotone2 (@euttF' E R eutt).
-Proof. repeat intro. eauto using euttF'_mon. Qed.
-Hint Resolve monotone_euttF' : paco.
-
-Lemma monotone_eutt'_ {E R} : monotone2 (@eutt'_ E R).
-Proof. red. eauto using euttF'_mon, paco2_mon_gen. Qed.
-Hint Resolve monotone_eutt'_ : paco.
-
-Lemma eutt__is_eutt'_ {E R} r (t1 t2: itree E R) :
-  eutt_ eq r t1 t2 <-> eutt'_ r t1 t2.
-Proof.
-  split; intros.
-  { revert t1 t2 H. pcofix CIH'. intros. destruct H0.
-    genobs t1 ot1. genobs t2 ot2. clear Heqot1 t1 Heqot2 t2.
-    assert (EM: notauF ot1 \/ notauF ot2 \/ ~(notauF ot1 \/ notauF ot2))
-      by (destruct ot1, ot2; simpl; tauto).
-    destruct EM as [EM|[EM|EM]].
-    - destruct FIN as [FIN _].
-      hexploit FIN; eauto 7. clear FIN; intro FIN.
-      destruct FIN as [ot' [UNTAUS NOTAU]].
-      hexploit EQV; eauto. intros EQNT.
-      induction UNTAUS; subst.
-      { pfold. inv EQNT; eauto. }
-      hexploit IHUNTAUS; eauto.
-      { intros. destruct UNTAUS1.
-        dependent destruction H; [|subst; contradiction].
-        hexploit @unalltaus_injective; [|econstructor|]; eauto. intros; subst; eauto.
-      }
-      intros EUTT. punfold EUTT.
-    - destruct FIN as [_ FIN].
-      hexploit FIN; eauto 7. clear FIN; intro FIN.
-      destruct FIN as [ot' [UNTAUS NOTAU]].
-      hexploit EQV; eauto. intros EQNT.
-      induction UNTAUS; subst.
-      { pfold. inv EQNT; eauto. }
-      hexploit IHUNTAUS; eauto.
-      { intros. destruct UNTAUS2.
-        dependent destruction H; [|subst; contradiction].
-        hexploit @unalltaus_injective; [|econstructor|]; eauto. intros; subst; eauto.
-      }
-      intros EUTT. punfold EUTT.
-    - destruct ot1, ot2; simpl in *; try tauto.
-      pfold. econstructor. right. apply CIH'.
-      econstructor.
-      + rewrite !finite_taus_tau in FIN. eauto.
-      + eauto using unalltaus_tau'.
-  }
-  { punfold H. econstructor; intros.
-    - split; intros.
-      + genobs t1 ot1. genobs t2 ot2. clear Heqot1 t1 Heqot2 t2.
-        destruct H0 as [ot' [UNTAUS NOTAU]].
-        move UNTAUS before r. revert_until UNTAUS.
-        induction UNTAUS; intros.
-        * induction H; eauto; try contradiction.
-          rewrite finite_taus_tau. eauto.
-        * induction H; eauto 7; try inv OBS; pclearbot
-          ; rewrite ?finite_taus_tau; eauto; eapply IHUNTAUS; eauto.
-          punfold EQTAUS.
-     + genobs t1 ot1. genobs t2 ot2. clear Heqot1 t1 Heqot2 t2.
-       destruct H0 as [ot' [UNTAUS NOTAU]].
-       move UNTAUS before r. revert_until UNTAUS.
-       induction UNTAUS; intros.
-       * induction H; eauto; try contradiction.
-         rewrite finite_taus_tau. eauto.
-       * induction H; eauto 7; try inv OBS; pclearbot
-         ; rewrite ?finite_taus_tau; eauto; eapply IHUNTAUS; eauto.
-         punfold EQTAUS.
-    - genobs t1 ot1. genobs t2 ot2. clear Heqot1 t1 Heqot2 t2.
-      destruct UNTAUS1 as [UNTAUS1 NT1]. destruct UNTAUS2 as [UNTAUS2 NT2].
-      move UNTAUS2 before r. move UNTAUS1 before r. revert_until UNTAUS1.
-      induction UNTAUS1.
-      + induction 1; intros.
-        * inv H; try contradiction; eauto.
-        * subst. inv H; try contradiction. eauto.
-      + induction 1; intros; subst.
-        * inv H; try contradiction; eauto.
-        * inv H; try contradiction; eauto.
-          pclearbot. eapply IHUNTAUS1; eauto.
-          punfold EQTAUS.
-  }
-Qed.
-
-Lemma eutt_is_eutt' {E R} r (t1 t2: itree E R) :
-  paco2 (eutt_ eq) r t1 t2 <-> paco2 eutt'_ r t1 t2.
-Proof.
-  split; intros; eapply paco2_mon_gen; eauto; intros; apply eutt__is_eutt'_; eauto.
-Qed.
-
-Lemma eutt_is_eutt'_gres {E R} r (t1 t2: itree E R) :
-  paco2 (eutt_ eq ∘ gres2 (eutt_ eq)) r t1 t2 <-> paco2 (eutt'_ ∘ gres2 eutt'_) r t1 t2.
-Proof.
-  split; intros.
-  - eapply paco2_mon_gen; eauto. intros.
-    red in PR|-*. rewrite <-eutt__is_eutt'_.
-    eapply monotone_eutt_; eauto. intros.
-    eapply grespectful2_impl; eauto. intros.
-    rewrite eutt__is_eutt'_. reflexivity.
-  - eapply paco2_mon_gen; eauto. intros.
-    red in PR|-*. rewrite eutt__is_eutt'_.
-    eapply monotone_eutt'_; eauto. intros.
-    eapply grespectful2_impl; eauto. intros.
-    rewrite eutt__is_eutt'_. reflexivity.
-Qed.
-
-Global Instance eutt'_paco {E R} r:
-  Proper (eutt eq ==> eutt eq ==> flip impl)
-         (paco2 (@eutt'_ E R ∘ gres2 eutt'_) r).
-Proof.
-  repeat intro.
-  rewrite <-eutt_is_eutt'_gres.
-  rewrite <-eutt_is_eutt'_gres in H1.
-  rewrite H, H0. eauto.
-Qed.
-
-Global Instance eutt'_gres {E R} r:
-  Proper (eutt eq ==> eutt eq ==> flip impl)
-         (gres2 (@eutt'_ E R) r).
-Proof.
-  repeat intro.
-  rewrite grespectful2_iff; [|intros; erewrite eutt__is_eutt'_; reflexivity].
-  rewrite grespectful2_iff in H1; [|intros; erewrite eutt__is_eutt'_; reflexivity].
-  rewrite H, H0. eauto.
+  pfold. pfold. econstructor. reflexivity.
 Qed.
