theories/MorphismsFacts.v
@@ -61,26 +61,22 @@ Definition interp_u {E F} (f : E ~> itree F) R :
           (fun _ e k => Tau (ITree.bind (f _ e)
                                         (fun x => interp f _ (k x)))).
 
-Lemma interp_unfold {E F R} {f : E ~> itree F} (t : itree E R) :
-  observe (interp f _ t) = observe (interp_u f _ (observe t)).
-Proof. eauto. Qed.
-
 Lemma unfold_interp {E F R} {f : E ~> itree F} (t : itree E R) :
-  interp f _ t ≅ interp_u f _ (observe t).
-Proof. rewrite itree_eta_, interp_unfold, <-itree_eta_. reflexivity. Qed.
+  observing eq (interp f _ t) (interp_u f _ (observe t)).
+Proof. econstructor. reflexivity. Qed.
 
 (** ** [interp] and constructors *)
 
 Lemma ret_interp {E F R} {f : E ~> itree F} (x: R):
-  interp f _ (Ret x) ≅ Ret x.
+  observing eq (interp f _ (Ret x)) (Ret x).
 Proof. rewrite unfold_interp. reflexivity. Qed.
 
 Lemma tau_interp {E F R} {f : E ~> itree F} (t: itree E R):
-  interp f _ (Tau t) ≅ Tau (interp f _ t).
+  observing eq (interp f _ (Tau t)) (Tau (interp f _ t)).
 Proof. rewrite unfold_interp. reflexivity. Qed.
 
 Lemma vis_interp {E F R} {f : E ~> itree F} U (e: E U) (k: U -> itree E R) :
-  interp f _ (Vis e k) ≅ Tau (ITree.bind (f _ e) (fun x => interp f _ (k x))).
+  observing eq (interp f _ (Vis e k)) (Tau (ITree.bind (f _ e) (fun x => interp f _ (k x)))).
 Proof. rewrite unfold_interp. reflexivity. Qed.
 
 (** ** [interp] properness *)
@@ -95,15 +91,15 @@ Proof.
   pcofix CIH.
   rename r into rr.
   intros l r Hlr.
-  rewrite itree_eta, (itree_eta (interp g _ r)), !interp_unfold.
+  rewrite itree_eta, (itree_eta (interp g _ r)), !unfold_interp.
   punfold Hlr; red in Hlr.
   destruct Hlr; pclearbot.
   - pupto2_final. pfold. red. cbn. eauto.
   - pupto2_final. pfold. red. cbn. eauto.
-  - pfold. econstructor. pupto2 (eq_itree_clo_bind F R).
-    constructor.
+  - pfold. econstructor. pupto2 eq_itree_clo_bind.
+    econstructor.
     + eapply Hfg.
-    + eauto. intros; pupto2_final; right; eauto.
+    + intros; subst; pupto2_final; right; eauto.
 Qed.
 
 Global Instance Proper_interp_eq_itree {E F R f}
@@ -118,8 +114,26 @@ Instance eutt_interp (E F : Type -> Type) (R : Type) :
   Proper (Rhom (fun _ => eutt eq) ==> eutt eq ==> eutt eq)
          (fun f => @interp E F f R).
 Proof.
-  (* this is going to be a terrible proof. *)
-Admitted.
+  repeat intro. revert_until H. repeat red in H.
+  cut (forall T t1 t2 k1 k2 (EQt: t1 ≈ t2) (EQk: forall v:T, k1 v ≈ k2 v),
+          (v <- t1 ;; interp x R (k1 v)) ≈ (v <- t2 ;; interp y R (k2 v))).
+  { intros.
+    hexploit (H0 _ (Ret ()) (Ret ()) (fun _ => x0) (fun _ => y0)); try reflexivity; eauto. intros EQV.
+    rewrite !ret_bind in EQV. eauto.
+  }
+
+  pcofix CIH. intros.
+  pfold. revert_until CIH. pcofix CIH'. intros.
+  do 2 punfold EQt. pfold.
+  rewrite !unfold_bind. genobs_clear t1 ot1. genobs_clear t2 ot2.
+  induction EQt; intros; subst; pclearbot; try (econstructor; eauto 7; fail).
+  simpl. rewrite !unfold_interp. unfold interp_u. unfold handleF.
+  specialize (EQk r2). do 2 punfold EQk.
+  genobs (k1 r2) kr1. genobs (k2 r2) kr2. clear Heqkr1 k1 Heqkr2 k2 r2.
+  induction EQk; intros; subst; pclearbot; try (econstructor; eauto 7; fail).
+  econstructor. right.
+  eapply (CIH' _ (Ret ()) (Ret ()) (fun _ => t1) (fun _ => t2)); try reflexivity; eauto.
+Qed.
 
 Lemma interp_ret : forall {E F R} x
       (f : E ~> itree F),
@@ -139,14 +153,14 @@ Proof.
   pcofix CIH. intros.
   rewrite (itree_eta t). destruct (observe t).
   (* TODO: [ret_bind] (0.8s) is much slower than [ret_bind_] (0.02s) *)
-  - rewrite ret_interp. rewrite !ret_bind_. pupto2_final. apply reflexivity.
-  - rewrite tau_interp, !tau_bind_, tau_interp.
+  - rewrite ret_interp. rewrite !ret_bind. pupto2_final. apply reflexivity.
+  - rewrite tau_interp, !tau_bind, tau_interp.
     pupto2_final. pfold. econstructor. eauto.
   - rewrite vis_interp, tau_bind. rewrite bind_bind.
     pfold. do 2 red; cbn. constructor.
     pupto2 (eq_itree_clo_bind F S). econstructor.
     + reflexivity.
-    + intros; specialize (CIH _ (k0 v) k); auto.
+    + intros; subst. specialize (CIH _ (k0 u2) k); auto.
 Qed.
 
 
@@ -158,7 +172,7 @@ Proof.
   unfold ITree.liftE. rewrite vis_interp.
   apply itree_eq_tau.
   assert (pointwise_relation _ (@eq_itree _ _ _ (@eq R)) (fun x : R => interp f R (Ret x)) (fun x => Ret x)).
-  {red. intros. apply ret_interp. }
+  {red. intros. rewrite ret_interp. reflexivity. }
   rewrite H. rewrite bind_ret.
   reflexivity.
 Qed.
@@ -174,19 +188,17 @@ Proof.
   pcofix CIH.
   intros t.
   rewrite unfold_interp. unfold interp_u. unfold handleF.
-  rewrite eutt_is_eutt'_gres.
   pfold. revert t. pcofix CIH'.
   intros t.
-  destruct (observe t); cbn.
+  destruct (observe t); cbn; eauto.
   - pfold. econstructor.
-  - pfold. econstructor.
-    right. rewrite interp_unfold. unfold interp_u. unfold handleF.
+    right. rewrite unfold_interp. unfold interp_u. unfold handleF.
     apply CIH'.
   - pfold. econstructor. cbn. econstructor. intros.
     assert (ITree.bind' (fun x0 : u => interp (fun (T : Type) (e0 : E T) => ITree.liftE e0) R (k x0)) (Ret x) = (x0 <- Ret x ;; interp (fun (T : Type) (e0 : E T) => ITree.liftE e0) R (k x0))).
     { intros; reflexivity. }
     rewrite H.
-    rewrite ret_bind_. (* TODO: Why does [ret_bind] not work at all. *)
+    rewrite ret_bind.
     pupto2_final. right. apply CIH.
 Qed.
 
@@ -210,132 +222,11 @@ Proof.
   - pupto2_final. pfold. econstructor. right.  apply CIH.
   - rewrite interp_bind.
     pfold. econstructor.
-    pupto2 eq_itree_clo_bind_h.
+    pupto2 eq_itree_clo_bind.
     apply pbc_intro_h with (RU := eq).
     + reflexivity.
     + intros.
       pupto2_final. right. subst. apply CIH.
-Qed.
-
-(** * [interp1] *)
-
-(* SAZ: If we need to introduce these auxilliar definitions to prove
-   properties about functions like interp1, I think that we should
-   _define_ interp1 in terms of its unfolding.  I have experimented
-   with porting interp_state and interp1_state to this form.
-*)
-(* Unfolding of [interp1]. *)
-Definition interp1_u {E F G} `{F -< G} (h : E ~> itree G) R :
-  itreeF (E +' F) R _ -> itree G R :=
-  handleF (interp1 h _)
-          (fun _ ef k =>
-             match ef with
-             | inl1 e => Tau (ITree.bind (h _ e)
-                                         (fun x => interp1 h _ (k x)))
-             | inr1 f => Vis (subeffect _ f) (fun x => interp1 h _ (k x))
-             end).
-
-Lemma interp1_unfold {E F G} `{F -< G} {R} {f : E ~> itree G} (t : itree (E +' F) R) :
-  observe (interp1 f _ t) = observe (interp1_u f _ (observe t)).
-Proof. eauto. Qed.
-
-Lemma unfold_interp1 {E F G} `{F -< G} {R} {f : E ~> itree G} (t : itree (E +' F) R) :
-  interp1 f _ t ≅ interp1_u f _ (observe t).
-Proof. rewrite itree_eta, interp1_unfold, <-itree_eta. reflexivity. Qed.
-
-(** ** [interp1] is equivalent to [interp] *)
-
-Section interp1_is_interp.
-
-Context {E F G : Type -> Type} `{F -< G} (f : E ~> itree G).
-
-Definition interp_match : (E +' F) ~> itree G :=
-  fun _ ef => match ef with inl1 e => f _ e | inr1 e => Vis (subeffect _ e) (fun r => Ret r) end.
-
-Inductive interp_inv {R} : relation (itree' G R) :=
-| _interp_inv_main t:
-    interp_inv
-      (observe (interp interp_match _ t)) (observe (interp1 f _ t))
-| _interp_inv_bind u t (k: u -> _):
-    interp_inv
-      (observe (ITree.bind t (fun x => interp interp_match _ (k x))))
-      (observe (ITree.bind t (fun x => interp1 f _ (k x))))
-.
-Hint Constructors interp_inv.
-
-Lemma interp_inv_main_step R (t: itree _ R) :
-  euttF' (fun x y => interp_inv (observe x) (observe y)) interp_inv
-         (observe (interp interp_match _ t)) (observe (interp1 f _ t)).
-Proof.
-  rewrite interp_unfold, interp1_unfold.
-  genobs t ot. clear Heqot t.
-  destruct ot; simpl; eauto.
-  destruct e; simpl; eauto.
-  econstructor. rewrite unfold_bind.
-  econstructor. intros.
-  fold_bind. rewrite unfold_bind. simpl. eauto.
-Qed.
-
-Lemma interp_is_interp1 R (t: itree _ R) :
-  interp interp_match _ t ≈ interp1 f _ t.
-Proof.
-  revert t.
-  cut (forall (t1 t2: itree _ R) (REL: interp_inv (observe t1) (observe t2)), t1 ≈ t2).
-  { eauto. }
-
-  intros. apply eutt_is_eutt'.
-  revert t1 t2 REL. pcofix CIH. intros. pfold.
-  revert t1 t2 REL. pcofix CIH'. intros.
-  destruct REL.
-  - pfold. eapply euttF'_mon; eauto using interp_inv_main_step; intros.
-    eapply upaco2_mon; eauto. intros.
-    eapply (CIH' (go x2) (go x3)); eauto.
-  - rewrite !unfold_bind. fold_bind.
-    genobs t ot. clear Heqot t.
-    destruct ot; simpl; eauto 10.
-    pfold. eapply euttF'_mon; eauto using interp_inv_main_step; intros.
-    eapply upaco2_mon; eauto. intros.
-    eapply (CIH' (go x2) (go x3)); eauto.
-Qed.
-
-End interp1_is_interp.
-
-Lemma eq_itree_interp1_ {E F R} (h1 h2 : E ~> itree F) :
-  (forall T (e : E T), h1 _ e ≅ h2 _ e) ->
-  forall t1 t2 : itree (E +' F) R,
-    t1 ≅ t2 -> interp1 h1 _ t1 ≅ interp1 h2 _ t2.
-Proof.
-  intros Hh t1 t2 Ht.
-  pupto2_init. revert_until R.
-  pcofix CIH. intros.
-  rewrite !unfold_interp1.
-  punfold Ht; red in Ht.
-  destruct Ht; pclearbot.
-  - pupto2_final. pfold. red. cbn. eauto.
-  - pupto2_final. pfold. red. cbn. eauto.
-  - pfold. destruct e; cbn; econstructor.
-    + pupto2 (eq_itree_clo_bind F R).
-      constructor.
-      * auto.
-      * intros; pupto2_final; eauto.
-    + intros; pupto2_final; eauto.
-Qed.
-
-Instance eq_itree_interp1 {E F G} `{F -< G} {R} (h : E ~> itree F) :
-  Proper (@eq_itree (E +' F) _ _ eq ==> eq_itree eq) (interp1 h R).
-Proof.
-  repeat intro.
-  eapply eq_itree_interp1_; auto.
-  reflexivity.
-Qed.
-
-Instance eutt_interp1 {E F G: Type -> Type} `{F -< G} (h: E ~> itree G) R:
-  Proper (eutt eq ==> eutt eq) (@interp1 E F G _ h R).
-Proof.
-  repeat intro.
-  rewrite <- 2 interp_is_interp1.
-  eapply eutt_interp; auto.
-  red; reflexivity.
 Qed.
 
 (** * [interp_state] *)
@@ -362,9 +253,9 @@ Proof.
   - pupto2_final. pfold. red. cbn. subst. eauto.
   - pupto2_final. pfold. red. cbn. subst. eauto.
   - pfold. econstructor. pupto2 (eq_itree_clo_bind F (S * R)).
-    constructor.
+    econstructor.
     + subst. reflexivity.
-    + intros; pupto2_final; right; eauto.
+    + intros; subst. pupto2_final; right; eauto.
 Qed.
 
 
@@ -391,9 +282,9 @@ Proof.
   - pfold.
     destruct e.
     * econstructor. pupto2 (eq_itree_clo_bind F (S * R)).
-      constructor.
+      econstructor.
       + subst. reflexivity.
-      + intros. pupto2_final. right. eauto.
+      + intros; subst. pupto2_final. right. eauto.
     * econstructor. intros. pupto2_final. right.
       eauto.
 Qed.
@@ -514,15 +405,15 @@ Proof.
   rewrite (itree_eta t).
   destruct (observe t).
   (* TODO: performance issues with [ret|tau|vis_bind] here too. *)
-  - cbn. rewrite interp_state_ret. rewrite !ret_bind_. simpl.
+  - cbn. rewrite interp_state_ret. rewrite !ret_bind. simpl.
     pupto2_final. apply reflexivity.
-  - cbn. rewrite interp_state_tau, !tau_bind_, interp_state_tau.
+  - cbn. rewrite interp_state_tau, !tau_bind, interp_state_tau.
     pupto2_final. pfold. econstructor. right. apply CIH.
-  - cbn. rewrite interp_state_vis, tau_bind_, vis_bind_, bind_bind, interp_state_vis.
+  - cbn. rewrite interp_state_vis, tau_bind, vis_bind, bind_bind, interp_state_vis.
     pfold. red. constructor.
     pupto2 (eq_itree_clo_bind F (S * B)). econstructor.
     + reflexivity.
-    + intros. specialize (CIH _ (k0 (snd v)) k (fst v)). auto.
+    + intros. subst. specialize (CIH _ (k0 (snd u2)) k (fst u2)). auto.
 Qed.
 
 Lemma interp1_state_bind {E F : Type -> Type} {A B S : Type}
@@ -539,17 +430,17 @@ Proof.
   intros A t k s.
   rewrite (itree_eta t).
   destruct (observe t).
-  - cbn. rewrite interp1_state_ret. rewrite !ret_bind_. simpl.
+  - cbn. rewrite interp1_state_ret. rewrite !ret_bind. simpl.
     pupto2_final. apply reflexivity.
-  - cbn. rewrite interp1_state_tau, !tau_bind_, interp1_state_tau.
+  - cbn. rewrite interp1_state_tau, !tau_bind, interp1_state_tau.
     pupto2_final. pfold. econstructor. right. apply CIH.
   - cbn. destruct e.
-    * rewrite interp1_state_vis1, tau_bind_, vis_bind_, bind_bind, interp1_state_vis1.
+    * rewrite interp1_state_vis1, tau_bind, vis_bind, bind_bind, interp1_state_vis1.
       pfold. red. constructor.
       pupto2 (eq_itree_clo_bind F (S * B)). econstructor.
       + reflexivity.
-      + intros. specialize (CIH _ (k0 (snd v)) k (fst v)). auto.
-   * rewrite interp1_state_vis2, !vis_bind_. rewrite itree_eta. rewrite unfold_interp1_state.
+      + intros. subst. specialize (CIH _ (k0 (snd u2)) k (fst u2)). auto.
+   * rewrite interp1_state_vis2, !vis_bind. rewrite itree_eta. rewrite unfold_interp1_state.
      cbn. pfold. constructor. intros.
      specialize (CIH _ (k0 v) k s). auto.
 Qed.
@@ -581,7 +472,7 @@ Proof.
     pupto2 eq_itree_clo_bind.
     econstructor.
     + reflexivity.
-    + intros. pupto2_final. right. apply CIH.
+    + intros. subst. pupto2_final. right. apply CIH.
 Qed.
 
 Lemma translate_to_interp {E F R} (f : E ~> F) (t : itree E R) :
@@ -596,14 +487,12 @@ Proof.
   rewrite unfold_translate.
   rewrite unfold_interp.
   unfold translateF, interp_u, handleF.
-  rewrite eutt_is_eutt'_gres.
   pfold. revert t. pcofix CIH'.
   intros t.
-  destruct (observe t).
-  - pfold. econstructor.
+  destruct (observe t); cbn; eauto.
   - pfold. econstructor.
     right. rewrite unfold_translate. unfold translateF.
-    rewrite interp_unfold. unfold interp_u. apply CIH'.
+    rewrite unfold_interp. unfold interp_u. apply CIH'.
   - pfold. econstructor. unfold ITree.liftE. rewrite vis_bind.
     econstructor. intros.
     rewrite (itree_eta (x0 <- Ret x;; interp (fun (T : Type) (e0 : E T) => Vis (f T e0) (fun x1 : T => Ret x1)) R (k x0))).
@@ -631,18 +520,16 @@ Proof.
   pcofix CIH.
   intros t.
   rewrite unfold_interp. unfold interp_u. unfold handleF.
-  rewrite eutt_is_eutt'_gres.
   pfold. revert t. pcofix CIH'.
   intros t.
-  destruct (observe t); cbn.
+  destruct (observe t); cbn; eauto.
   - pfold. econstructor.
-  - pfold. econstructor.
-    right. rewrite interp_unfold. unfold interp_u. unfold handleF.
+    right. rewrite unfold_interp. unfold interp_u. unfold handleF.
     apply CIH'.
   - pfold. econstructor. cbn. econstructor. intros.
     assert (ITree.bind' (fun x0 : u => interp eh_id R (k x0)) (Ret x) = (x0 <- Ret x ;; interp eh_id R (k x0))).
     { intros; reflexivity. }
-    rewrite H. rewrite ret_bind_. (* TODO: [ret_bind] doesn't work *)
+    rewrite H. rewrite ret_bind. (* TODO: [ret_bind] doesn't work *)
     pupto2_final. right. apply CIH.
 Qed.
 
@@ -737,21 +624,122 @@ Proof.
   simpl. unfold Sum1.idE. reflexivity.
 Qed.
 
+(***
+ lemmas about [interp1].
+ We can remove [interp1] but keep it just in case it is useful.
+ ***)
+
+Definition interp1_u {E F G} `{F -< G} (h : E ~> itree G) R :
+  itreeF (E +' F) R _ -> itree G R :=
+  handleF (interp1 h _)
+          (fun _ ef k =>
+             match ef with
+             | inl1 e => Tau (ITree.bind (h _ e)
+                                         (fun x => interp1 h _ (k x)))
+             | inr1 f => Vis (subeffect _ f) (fun x => interp1 h _ (k x))
+             end).
+
+Lemma unfold_interp1 {E F G : Type -> Type} `{F -< G} (h : E ~> itree G) R (t : itree (E +' F) R) :
+  observing eq (interp1 h _ t) (interp1_u h _ (observe t)).
+Proof. econstructor. auto. Qed.
+
+Lemma unfold_interp1_ {E F G : Type -> Type} `{F -< G} (h : E ~> itree G) R (t : itree (E +' F) R) :
+  interp1 h _ t ≅ interp1_u h _ (observe t).
+Proof. rewrite itree_eta, unfold_interp1, <-itree_eta. reflexivity. Qed.
+
+(** ** [interp1] is equivalent to [interp] *)
+
+Definition interp_match {E F} (f: E ~> itree F) : (E +' F) ~> itree F :=
+  fun _ ef => match ef with inl1 e => f _ e | inr1 e => Vis e (fun r => Ret r) end.
+
+Inductive interp_inv {E F R} (f: E ~> itree F) : relation (itree' F R) :=
+| _interp_inv_main t:
+    interp_inv f
+      (observe (interp (interp_match f) _ t)) (observe (interp1 f _ t))
+| _interp_inv_bind u t (k: u -> _):
+    interp_inv f
+      (observe (ITree.bind t (fun x => interp (interp_match f) _ (k x))))
+      (observe (ITree.bind t (fun x => interp1 f _ (k x))))
+.
+Hint Constructors interp_inv.
+
+Lemma interp_inv_main_step E F R (f: E ~> itree F) (t: itree _ R) :
+  euttF eq (fun x y => interp_inv f (observe x) (observe y)) (interp_inv f)
+           (observe (interp (interp_match f) _ t)) (observe (interp1 f _ t)).
+Proof.
+  rewrite unfold_interp, unfold_interp1.
+  genobs_clear t ot.
+  destruct ot; simpl; eauto.
+  destruct e; simpl; eauto.
+  econstructor. rewrite unfold_bind.
+  econstructor. intros.
+  fold_bind. rewrite unfold_bind. simpl. eauto.
+Qed.
+
+Lemma interp_is_interp1 E F R (f: E ~> itree F) (t: itree _ R) :
+  interp (interp_match f) _ t ≈ interp1 f _ t.
+Proof.
+  revert t.
+  cut (forall (t1 t2: itree _ R) (REL: interp_inv f (observe t1) (observe t2)), t1 ≈ t2).
+  { eauto. }
+
+  intros. revert_until f. pcofix CIH. intros.
+  pfold. revert_until CIH. pcofix CIH'. intros.
+  destruct REL.
+  - pfold. eapply euttF_mon; eauto using interp_inv_main_step; intros.
+    eapply upaco2_mon; eauto. intros.
+    eapply (CIH' (go x2) (go x3)); eauto.
+  - rewrite !unfold_bind. fold_bind.
+    genobs_clear t ot. 
+    destruct ot; simpl; eauto 10.
+    pfold. eapply euttF_mon; eauto using interp_inv_main_step; intros.
+    eapply upaco2_mon; eauto. intros.
+    eapply (CIH' (go x2) (go x3)); eauto.
+Qed.
+
+Instance eq_itree_interp1 {E F R} (h : E ~> itree F) :
+  Proper (@eq_itree (E +' F) _ _ eq ==> eq_itree eq) (interp1 h R).
+Proof.
+  repeat intro. pupto2_init. revert_until R.
+  pcofix CIH. intros.
+  rewrite !unfold_interp1_.
+  punfold H0; red in H0.
+  destruct H0; pclearbot.
+  - pupto2_final. pfold. red. cbn. eauto.
+  - pupto2_final. pfold. red. cbn. eauto.
+  - pfold. destruct e; cbn; econstructor.
+    + pupto2 (eq_itree_clo_bind F R).
+      econstructor.
+      * reflexivity.
+      * intros; subst. pupto2_final; eauto.
+    + intros. pupto2_final. eauto.
+Qed.
+
+Instance eutt_interp1 {E F: Type -> Type} (h: E ~> itree F) R:
+  Proper (eutt eq ==> eutt eq) (@interp1 E F F _ h R).
+Proof.
+  repeat intro.
+  rewrite <- 2 interp_is_interp1.
+  eapply eutt_interp; auto.
+  red; reflexivity.
+Qed.
+
 Lemma interp1_bind {E F G} `{F -< G} {R S} (h : E ~> itree G) (t : _ R) (k : _ -> itree (E +' F) S) :
   interp1 h _ (t >>= k) ≅ interp1 h _ t >>= fun x => interp1 h _ (k x).
 Proof.
   pupto2_init.
   revert t; pcofix self; intros.
-  rewrite 2 unfold_interp1. rewrite unfold_bind.
+  rewrite !unfold_interp1_, unfold_bind, unfold_bind_.
   destruct (observe t); cbn.
-  - rewrite ret_bind_. rewrite <- unfold_interp1.
-    pupto2_final. apply RelationClasses.reflexivity.
-  - rewrite tau_bind_. pfold; constructor; auto.
-  - destruct e.
-    + rewrite tau_bind_. rewrite bind_bind. pfold; constructor.
-      pupto2 eq_itree_clo_bind. constructor.
-      reflexivity. auto.
-    + rewrite vis_bind_. pfold; constructor; auto.
+  - rewrite unfold_interp1_.
+    pupto2_final. apply reflexivity.
+  - pfold; constructor; auto.
+  - destruct e; cbn.
+    + rewrite bind_bind. pfold; constructor.
+      pupto2 eq_itree_clo_bind. econstructor.
+      * reflexivity.
+      * intros; subst. eauto.
+    + pfold; constructor; auto.
 Qed.
 
 Lemma translate_interp1 {E F R} (h : F ~> itree E) :
@@ -760,7 +748,7 @@ Lemma translate_interp1 {E F R} (h : F ~> itree E) :
 Proof.
   pcofix self; intros.
   pfold; red.
-  rewrite interp1_unfold.
+  rewrite unfold_interp1.
   rewrite TranslateFacts.unfold_translate.
   destruct (observe t); cbn; auto.
 Qed.
@@ -770,9 +758,9 @@ Lemma interp1_liftE {E F G: Type -> Type} `{F -< G}:
     @interp1 E F G _ h T (lift e) ≈ h T e.
 Proof.
   intros. unfold lift.
-  rewrite unfold_interp1; cbn.
+  rewrite unfold_interp1_; cbn.
   rewrite tau_eutt.
-  setoid_rewrite unfold_interp1; cbn.
+  setoid_rewrite unfold_interp1_; cbn.
   rewrite bind_ret.
   reflexivity.
 Qed.
