theories/Eq/UpToTausExplicit.v
@@ -1,0 +1,744 @@
+(* Equivalence up to taus *)
+(* We consider tau as an "internal step", that should not be
+   visible to the outside world, so adding or removing [Tau]
+   constructors from an itree should produce an equivalent itree.
+
+   We must be careful because there may be infinite sequences of
+   taus (i.e., [spin]). Here we shall only allow inserting finitely
+   many taus between any two visible steps ([Ret] or [Vis]), so that
+   [spin] is only related to itself. The main consequence of this
+   choice is that equivalence up to taus is an equivalence relation.
+ *)
+
+(* TODO:
+   - Generalize Reflexivity, Symmetry, Transitivity to heterogeneous
+     eutt.
+   - Make eutt a notation instead of a definition?
+ *)
+
+Require Import Paco.paco.
+
+From Coq Require Import
+     Program
+     Lia
+     Classes.RelationClasses
+     Classes.Morphisms
+     Setoids.Setoid
+     Relations.Relations.
+
+From ITree Require Import
+     Core.
+
+From ITree Require Export
+     Eq.Eq
+     Eq.Untaus.
+
+Local Open Scope itree.
+
+Section EUTT.
+
+Context {E : Type -> Type} {R1 R2 : Type} (RR : R1 -> R2 -> Prop).
+
+(* Equivalence between visible steps of computation (i.e., [Vis] or
+   [Ret], parameterized by a relation [euttE] between continuations
+   in the [Vis] case. *)
+Variant eq_notauF {I J} (euttE : I -> J -> Prop)
+: itreeF E R1 I -> itreeF E R2 J -> Prop :=
+| Eutt_ret : forall r1 r2,
+    RR r1 r2 ->
+    eq_notauF euttE (RetF r1) (RetF r2)
+| Eutt_vis : forall u (e : E u) k1 k2,
+    (forall x, euttE (k1 x) (k2 x)) ->
+    eq_notauF euttE (VisF e k1) (VisF e k2).
+Hint Constructors eq_notauF.
+
+Lemma eq_notauF_vis_inv1 {I J} {euttE : I -> J -> Prop} {U}
+  ot (e : E U) k :
+  eq_notauF euttE ot (VisF e k) ->
+  exists k',
+    ot = VisF e k' /\ (forall x, euttE (k' x) (k x)).
+Proof.
+  intros. remember (VisF e k) as t.
+  inversion H; subst; try discriminate.
+  inversion H2; subst; auto_inj_pair2; subst; eauto.
+Qed.
+
+(*
+Variant eq_notauF' {I} (euttE : relation I)
+: relation (itreeF E R I) :=
+| Eutt_ret' : forall r, eq_notauF' euttE (RetF r) (RetF r)
+| Eutt_vis' : forall {u1 u2} (e1 : E u1) (e2 : E u2) k1 k2,
+    eq_dep _ E _ e1 _ e2 ->
+    (forall x1 x2, JMeq x1 x2 -> euttE (k1 x1) (k2 x2)) ->
+    eq_notauF' euttE (VisF e1 k1) (VisF e2 k2).
+Hint Constructors eq_notauF'.
+
+Lemma eq_notauF_eq_eq_notauF': forall I (euttE : relation I) t s,
+  eq_notauF euttE t s <-> eq_notauF' euttE t s.
+Proof.
+  split; intros EUTT; destruct EUTT; eauto.
+  - econstructor; intros; subst; eauto.
+  - assert (u1 = u2) by (inv H; eauto).
+    subst. apply eq_dep_eq in H. subst. eauto.
+Qed.
+*)
+
+(* [euttE_ euttE t1 t2] means that, if [t1] or [t2] ever takes a
+   visible step ([Vis] or [Ret]), then the other takes the same
+   step, and the subsequent continuations (in the [Vis] case) are
+   related by [euttE]. In particular, [(t1 = spin)%eq_itree] if
+   and only if [(t2 = spin)%eq_itree]. Note also that in that
+   case, the parameter [euttE] is irrelevant.
+
+   This is the relation we will take a fixpoint of. *)
+Inductive euttEF (euttE : itree E R1 -> itree E R2 -> Prop)
+          (ot1 : itreeF E R1 (itree E R1))
+          (ot2 : itreeF E R2 (itree E R2)) : Prop :=
+| euttEF_ (FIN: finite_tausF ot1 <-> finite_tausF ot2)
+         (EQV: forall ot1' ot2'
+                  (UNTAUS1: unalltausF ot1 ot1')
+                  (UNTAUS2: unalltausF ot2 ot2'),
+               eq_notauF euttE ot1' ot2')
+.
+Hint Constructors euttEF.
+
+Definition euttE_ (euttE : itree E R1 -> itree E R2 -> Prop)
+           (t1 : itree E R1) (t2 : itree E R2) : Prop :=
+  euttEF euttE (observe t1) (observe t2).
+Hint Unfold euttE_.
+
+(* Paco takes the greatest fixpoints of monotone relations. *)
+
+Lemma monotone_eq_notauF : forall I J (r r' : I -> J -> Prop) x1 x2
+      (IN: eq_notauF r x1 x2)
+      (LE: r <2= r'),
+    eq_notauF r' x1 x2.
+Proof. pmonauto. Qed.
+Hint Resolve monotone_eq_notauF.
+
+(* [euttE_] is monotone. *)
+Lemma monotone_euttE_ : monotone2 euttE_.
+Proof. pmonauto. Qed.
+Hint Resolve monotone_euttE_ : paco.
+
+(* We now take the greatest fixpoint of [euttE_]. *)
+
+(* Equivalence Up To Taus.
+
+   [euttE t1 t2]: [t1] is equivalent to [t2] up to taus. *)
+Definition euttE : itree E R1 -> itree E R2 -> Prop := paco2 euttE_ bot2.
+Hint Unfold euttE.
+
+Global Arguments euttE t1%itree t2%itree.
+
+(* Lemmas about the auxiliary relations. *)
+
+(* Many have a name [X_Y] to represent an implication
+   [X _ -> Y _] (possibly with more arguments on either side). *)
+
+(**)
+
+Lemma euttEF_tau r t1 t2 t1' t2'
+    (OBS1: TauF t1' = observe t1)
+    (OBS2: TauF t2' = observe t2)
+    (REL: euttE_ r t1' t2'):
+  euttE_ r t1 t2.
+Proof.
+  intros. destruct REL. econstructor.
+  - simpobs. rewrite !finite_taus_tau. eauto.
+  - intros. eapply EQV; eapply unalltaus_tau; eauto.
+Qed.
+
+Lemma euttEF_tau_left r t1 t2 t1'
+    (OBS: TauF t1 = observe t1')
+    (REL: euttE_ r t1' t2):
+  euttE_ r t1 t2.
+Proof.
+  intros. destruct REL. econstructor.
+  - rewrite <- FIN. symmetry. rewrite <- OBS. rewrite <- finite_taus_tau; eauto. reflexivity.
+  - intros. eapply EQV; eauto. rewrite <- OBS. inversion UNTAUS1. constructor; auto.
+    econstructor; eauto.
+Qed.
+
+Lemma euttEF_tau_right r t1 t2 t2'
+    (OBS: TauF t2 = observe t2')
+    (REL: euttE_ r t1 t2'):
+  euttE_ r t1 t2.
+Proof.
+  intros. destruct REL. econstructor.
+  - rewrite FIN. rewrite <- OBS. rewrite <- finite_taus_tau; eauto. reflexivity.
+  - intros. eapply EQV; eauto. rewrite <- OBS. inversion UNTAUS2. constructor; auto.
+    econstructor; eauto.
+Qed.
+
+Lemma euttEF_vis {u} (r : _ -> _ -> Prop) t1 t2 (e : _ u) k1 k2
+    (OBS1: VisF e k1 = observe t1)
+    (OBS2: VisF e k2 = observe t2)
+    (REL: forall x, r (k1 x) (k2 x)):
+  euttE_ r t1 t2.
+Proof.
+  intros. econstructor.
+  - split; intros; eapply notau_finite_taus; eauto.
+  - intros.
+    apply unalltaus_notau_id in UNTAUS1; eauto.
+    apply unalltaus_notau_id in UNTAUS2; eauto.
+    simpobs. subst. eauto.
+Qed.
+
+(**)
+
+Lemma euttE_strengthen :
+  forall r (t1 : itree E R1) (t2 : itree E R2)
+     (FIN: finite_taus t1 <-> finite_taus t2)
+     (EQV: forall t1' t2'
+              (UNT1: unalltaus t1 t1')
+              (UNT2: unalltaus t2 t2'),
+         paco2 (euttE_ ∘ gres2 euttE_) r t1' t2'),
+    paco2 (euttE_ ∘ gres2 euttE_) r t1 t2.
+Proof.
+  intros. pfold. econstructor; eauto.
+  intros.
+  hexploit (EQV (go ot1') (go ot2')); eauto.
+  intros EQV'. punfold EQV'. destruct EQV'.
+  eapply EQV0;
+    repeat constructor; eauto.
+Qed.
+
+(**)
+
+Lemma eq_unalltaus (t1 : itree E R1) (t2 : itree E R2) ot1'
+    (FT: unalltausF (observe t1) ot1')
+    (EQV: eq_itree RR t1 t2) :
+  exists ot2', unalltausF (observe t2) ot2'.
+Proof.
+  genobs t1 ot1. revert t1 Heqot1 t2 EQV.
+  destruct FT as [Huntaus Hnotau].
+  induction Huntaus; intros; punfold EQV; unfold_eq_itree; subst.
+  - eexists. constructor; eauto. inv EQV; simpl; eauto.
+  - inv EQV; simpobs; try inv Heqot1.
+    pclearbot. edestruct IHHuntaus as [? []]; eauto.
+Qed.
+
+Lemma eq_unalltaus_eqF (t : itree E R1) (s : itree E R2) ot'
+    (UNTAUS : unalltausF (observe t) ot')
+    (EQV: eq_itree RR t s) :
+  exists os', unalltausF (observe s) os' /\ eq_itreeF RR (eq_itree RR) ot' os'.
+Proof.
+  destruct UNTAUS as [Huntaus Hnotau].
+  remember (observe t) as ot. revert s t Heqot EQV.
+  induction Huntaus; intros; punfold EQV; unfold_eq_itree.
+  - eexists (observe s). split.
+    inv EQV; simpobs; eauto.
+    subst; eauto.
+    eapply eq_itreeF_mono; eauto.
+    intros ? ? [| []]; eauto.
+  - inv EQV; simpobs; inversion Heqot; subst.
+    destruct REL as [| []].
+    edestruct IHHuntaus as [? [[]]]; eauto 10.
+Qed.
+
+Lemma eq_unalltaus_eq (t : itree E R1) (s : itree E R2) t'
+    (UNTAUS : unalltausF (observe t) (observe t'))
+    (EQV: eq_itree RR t s) :
+  exists s', unalltausF (observe s) (observe s') /\ eq_itree RR t' s'.
+Proof.
+  eapply eq_unalltaus_eqF in UNTAUS; try eassumption.
+  destruct UNTAUS as [os' []]. eexists (go os'); split; eauto.
+  pfold. eapply eq_itreeF_mono; eauto.
+Qed.
+
+Lemma euttE_Ret x y :
+  RR x y -> euttE (Ret x) (Ret y).
+Proof.
+  intros; pfold.
+  constructor.
+  split; intros; eapply finite_taus_ret; reflexivity.
+  intros.
+  apply unalltausF_ret in UNTAUS1.
+  apply unalltausF_ret in UNTAUS2.
+  subst; constructor; assumption.
+Qed.
+
+Lemma euttE_Vis {U} (e: E U) k k' :
+  (forall x, euttE (k x) (k' x)) ->
+  euttE (Vis e k) (Vis e k').
+Proof.
+  intros.
+  pfold; constructor.
+  split; intros; eapply finite_taus_vis; reflexivity.
+  intros.
+  cbn in *.
+  apply unalltausF_vis in UNTAUS1.
+  apply unalltausF_vis in UNTAUS2.
+  subst; constructor.
+  intros x; specialize (H x).
+  punfold H.
+Qed.
+
+End EUTT.
+
+Hint Unfold euttE_.
+Hint Unfold euttE.
+Hint Resolve monotone_eq_notauF.
+Hint Constructors eq_notauF.
+Hint Constructors euttEF.
+Hint Resolve monotone_euttE_ : paco.
+
+(** *** [eq_notauF] lemmas *)
+
+Lemma eq_notauF_and {E R1 R2} (RR : R1 -> R2 -> Prop) {I J}
+        (euttE1 euttE2 euttE : I -> J -> Prop) :
+  (forall t1 t2, euttE1 t1 t2 -> euttE2 t1 t2 -> euttE t1 t2) ->
+  forall (ot1 : itreeF E R1 I) (ot2 : itreeF E R2 J),
+    eq_notauF RR euttE1 ot1 ot2 -> eq_notauF RR euttE2 ot1 ot2 ->
+    eq_notauF RR euttE ot1 ot2.
+Proof.
+  intros ? ? ? [] Hen2; inversion Hen2; auto.
+  auto_inj_pair2; subst; auto.
+Qed.
+
+Lemma eq_notauF_flip {E R1 R2} (RR : R1 -> R2 -> Prop) {I J}
+      (euttE : I -> J -> Prop) :
+  forall (ot1 : itreeF E R1 I) (ot2 : itreeF E R2 J),
+    eq_notauF (flip RR) (flip euttE) ot2 ot1 ->
+    eq_notauF RR euttE ot1 ot2.
+Proof.
+  intros ? ? []; auto.
+Qed.
+
+Delimit Scope euttE_scope with euttE.
+
+(** ** Generalized symmetry and transitivity *)
+
+Lemma Symmetric_eq_notauF_ {E R1 R2}
+      (RR1 : R1 -> R2 -> Prop) (RR2 : R2 -> R1 -> Prop)
+      {I J} (r1 : I -> J -> Prop) (r2 : J -> I -> Prop)
+      (SYM_RR : forall r1 r2, RR1 r1 r2 -> RR2 r2 r1)
+      (SYM_r : forall i j, r1 i j -> r2 j i)
+      (ot1 : itreeF E R1 I) (ot2 : itreeF E R2 J) :
+  eq_notauF RR1 r1 ot1 ot2 ->
+  eq_notauF RR2 r2 ot2 ot1.
+Proof. intros []; auto. Qed.
+
+Lemma Transitive_eq_notauF_ {E R1 R2 R3}
+      (RR1 : R1 -> R2 -> Prop) (RR2 : R2 -> R3 -> Prop)
+      (RR3 : R1 -> R3 -> Prop)
+      {I J K} (r1 : I -> J -> Prop) (r2 : J -> K -> Prop)
+      (r3 : I -> K -> Prop)
+      (TRANS_RR : forall r1 r2 r3, RR1 r1 r2 -> RR2 r2 r3 -> RR3 r1 r3)
+      (TRANS_r : forall i j k, r1 i j -> r2 j k -> r3 i k)
+      (ot1 : itreeF E R1 I) ot2 ot3 :
+  eq_notauF RR1 r1 ot1 ot2 ->
+  eq_notauF RR2 r2 ot2 ot3 ->
+  eq_notauF RR3 r3 ot1 ot3.
+Proof.
+  intros [] I2; inversion I2; eauto.
+  auto_inj_pair2; subst; eauto.
+Qed.
+
+Lemma Symmetric_euttEF_ {E R1 R2}
+      (RR1 : R1 -> R2 -> Prop) (RR2 : R2 -> R1 -> Prop)
+      (r1 : _ -> _ -> Prop) (r2 : _ -> _ -> Prop)
+      (SYM_RR : forall r1 r2, RR1 r1 r2 -> RR2 r2 r1)
+      (SYM_r : forall i j, r1 i j -> r2 j i)
+      (ot1 : itree' E R1) (ot2 : itree' E R2) :
+  euttEF RR1 r1 ot1 ot2 ->
+  euttEF RR2 r2 ot2 ot1.
+Proof.
+  intros []; split.
+  - split; apply FIN.
+  - intros. specialize (EQV _ _ UNTAUS2 UNTAUS1).
+    eapply Symmetric_eq_notauF_; eauto.
+Qed.
+
+Lemma Transitive_euttEF_ {E R1 R2 R3}
+      (RR1 : R1 -> R2 -> Prop) (RR2 : R2 -> R3 -> Prop)
+      (RR3 : R1 -> R3 -> Prop)
+      (r1 : _ -> _ -> Prop) (r2 : _ -> _ -> Prop)
+      (r3 : _ -> _ -> Prop)
+      (TRANS_RR : forall r1 r2 r3, RR1 r1 r2 -> RR2 r2 r3 -> RR3 r1 r3)
+      (TRANS_r : forall i j k, r1 i j -> r2 j k -> r3 i k)
+      (ot1 : itree' E R1) ot2 ot3 :
+  euttEF RR1 r1 ot1 ot2 ->
+  euttEF RR2 r2 ot2 ot3 ->
+  euttEF RR3 r3 ot1 ot3.
+Proof.
+  intros [] [].
+  constructor.
+  - etransitivity; eauto.
+  - intros t1' t3' H1 H3.
+    assert (FIN2 : finite_tausF ot2).
+    { apply FIN; eauto. }
+    destruct FIN2 as [t2' []].
+    eapply Transitive_eq_notauF_; eauto.
+Qed.
+
+Lemma Symmetric_euttE_ {E R1 R2}
+      (RR1 : R1 -> R2 -> Prop) (RR2 : R2 -> R1 -> Prop)
+      (r1 : _ -> _ -> Prop) (r2 : _ -> _ -> Prop)
+      (SYM_RR : forall r1 r2, RR1 r1 r2 -> RR2 r2 r1)
+      (SYM_r : forall i j, r1 i j -> r2 j i) :
+  forall (t1 : itree E R1) (t2 : itree E R2),
+    paco2 (euttE_ RR1) r1 t1 t2 -> paco2 (euttE_ RR2) r2 t2 t1.
+Proof.
+  pcofix self.
+  intros t1 t2 H12.
+  punfold H12.
+  pfold.
+  eapply Symmetric_euttEF_; try eassumption.
+  intros ? ? []; auto.
+Qed.
+
+Lemma Transitive_euttE_ {E R1 R2 R3}
+      (RR1 : R1 -> R2 -> Prop) (RR2 : R2 -> R3 -> Prop)
+      (RR3 : R1 -> R3 -> Prop)
+      (TRANS_RR : forall r1 r2 r3, RR1 r1 r2 -> RR2 r2 r3 -> RR3 r1 r3) :
+  forall (t1 : itree E R1) t2 t3,
+    euttE RR1 t1 t2 -> euttE RR2 t2 t3 -> euttE RR3 t1 t3.
+Proof.
+  pcofix self.
+  intros t1 t2 t3 H12 H23.
+  punfold H12; punfold H23; pfold.
+  eapply Transitive_euttEF_; try eassumption.
+  intros; pclearbot; eauto.
+Qed.
+
+Section EUTT_rel.
+
+Context {E : Type -> Type} {R : Type} (RR : R -> R -> Prop).
+
+(* Reflexivity of [eq_notauF], modulo a few assumptions. *)
+Lemma Reflexive_eq_notauF `{Reflexive _ RR} I (eq_ : I -> I -> Prop) :
+  Reflexive eq_ ->
+  forall (ot : itreeF E R I), notauF ot -> eq_notauF RR eq_ ot ot.
+Proof.
+  intros. destruct ot; try contradiction; econstructor; intros; subst; eauto.
+Qed.
+
+Global Instance Symmetric_eq_notauF `{Symmetric _ RR} I (eq_ : I -> I -> Prop) :
+  Symmetric eq_ -> Symmetric (@eq_notauF E _ _ RR _ _ eq_).
+Proof.
+  repeat intro. eapply Symmetric_eq_notauF_; eauto.
+Qed.
+
+Global Instance Transitive_eq_notauF `{Transitive _ RR} I (eq_ : I -> I -> Prop) :
+  Transitive eq_ -> Transitive (@eq_notauF E _ _ RR _ _ eq_).
+Proof.
+  repeat intro. eapply Transitive_eq_notauF_; eauto.
+Qed.
+
+Global Instance subrelation_eq_euttE :
+  @subrelation (itree E R) (eq_itree RR) (euttE RR).
+Proof.
+  pcofix CIH. intros.
+  pfold. econstructor.
+  { split; [|apply flip_eq_itree in H0]; intros; destruct H as [n [? ?]]; eauto using eq_unalltaus. }
+
+  intros. eapply eq_unalltaus_eqF in H0; eauto. destruct H0 as [s' [UNTAUS' EQV']].
+  hexploit @unalltaus_injective; [apply UNTAUS' | apply UNTAUS2 | intro X]; subst.
+  inv EQV'; simpobs; eauto.
+  eapply unalltaus_notau in UNTAUS1. contradiction.
+Qed.
+
+Global Instance Reflexive_euttEF `{Reflexive _ RR}
+       (r : itree E R -> itree E R -> Prop) :
+  Reflexive r -> Reflexive (euttEF RR r).
+Proof.
+  split.
+  - reflexivity.
+  - intros.
+    erewrite (unalltaus_injective _ _ _ UNTAUS1 UNTAUS2).
+    apply Reflexive_eq_notauF; eauto.
+Qed.
+
+Global Instance Symmetric_euttEF `{Symmetric _ RR}
+         (r : itree E R -> itree E R -> Prop) :
+  Symmetric r -> Symmetric (euttEF RR r).
+Proof.
+  intros SYM x y. apply Symmetric_euttEF_; auto.
+Qed.
+
+Global Instance Transitive_euttEF `{Transitive _ RR}
+       (r : itree E R -> itree E R -> Prop) :
+  Transitive r -> Transitive (euttEF RR r).
+Proof.
+  intros TRANS x y z. apply Transitive_euttEF_; auto.
+Qed.
+
+Global Instance Symmetric_euttE `{Symmetric _ RR}
+       (r : itree E R -> itree E R -> Prop)
+       (Sr : Symmetric r) :
+  Symmetric (paco2 (euttE_ RR) r).
+Proof. red; eapply Symmetric_euttE_; eauto. Qed.
+
+Global Instance Reflexive_euttE `{Reflexive _ RR}
+       (r : itree E R -> itree E R -> Prop) :
+  Reflexive (paco2 (euttE_ RR) r).
+Proof.
+  pcofix CIH.
+  intros. pfold. red. apply Reflexive_euttEF; eauto.
+Qed.
+
+End EUTT_rel.
+
+Section EUTT_eq.
+
+Context {E : Type -> Type} {R : Type}.
+
+Let euttE : itree E R -> itree E R -> Prop := euttE eq.
+
+Global Instance Transitive_euttE : Transitive euttE.
+Proof.
+  red; eapply Transitive_euttE_; eauto.
+  intros; subst; eauto.
+Qed.
+
+(**)
+
+(* [euttE] is preserved by removing one [Tau]. *)
+Lemma tauF_euttE (t t': itree E R) (OBS: TauF t' = observe t): euttE t t'.
+Proof.
+  pfold. split.
+  - simpobs. rewrite finite_taus_tau. reflexivity.
+  - intros t1' t2' H1 H2.
+    eapply unalltaus_tau in H1; eauto.
+    pose proof (unalltaus_injective _ _ _ H1 H2).
+    subst; apply Reflexive_eq_notauF; eauto.
+    left. apply reflexivity.
+Qed.
+
+Lemma tau_euttE (t: itree E R) : euttE (Tau t) t.
+Proof.
+  eapply tauF_euttE. eauto.
+Qed.
+
+(* [euttE] is preserved by removing all [Tau]. *)
+Lemma untaus_euttE (t t' : itree E R) : untausF (observe t) (observe t') -> euttE t t'.
+Proof.
+  intros H.
+  pfold. split.
+  - eapply untaus_finite_taus; eauto.
+  - induction H; intros.
+    + rewrite (unalltaus_injective _ _ _ UNTAUS1 UNTAUS2).
+      apply Reflexive_eq_notauF; eauto.
+      left; apply reflexivity.
+    + eapply unalltaus_tau in UNTAUS1; eauto.
+Qed.
+
+(* We can now rewrite with [euttE] equalities. *)
+Global Instance Equivalence_euttE : @Equivalence (itree E R) euttE.
+Proof. constructor; typeclasses eauto. Qed.
+
+(**)
+
+Global Instance euttE_go : Proper (going euttE ==> euttE) go.
+Proof. intros ? ? []; eauto. Qed.
+
+Global Instance euttE_observe : Proper (euttE ==> going euttE) observe.
+Proof.
+  constructor. punfold H. pfold. destruct H. econstructor; eauto.
+Qed.
+
+Global Instance euttE_tauF : Proper (euttE ==> going euttE) (fun t => TauF t).
+Proof.
+  constructor; pfold. punfold H.
+  destruct H. econstructor.
+  - split; intros; simpl.
+    + rewrite finite_taus_tau, <-FIN, <-finite_taus_tau; eauto.
+    + rewrite finite_taus_tau, FIN, <-finite_taus_tau; eauto.
+  - intros. eapply EQV; eapply unalltaus_tau; eauto.
+Qed.
+
+Global Instance euttE_VisF {u} (e: E u) :
+  Proper (pointwise_relation _ euttE ==> going euttE) (VisF e).
+Proof.
+  constructor; pfold. red in H. econstructor.
+  - repeat econstructor.
+  - intros.
+    destruct UNTAUS1 as [UNTAUS1 Hnotau1].
+    destruct UNTAUS2 as [UNTAUS2 Hnotau2].
+    dependent destruction UNTAUS1.
+    dependent destruction UNTAUS2. simpobs.
+    econstructor; intros; left; apply H.
+Qed.
+
+Global Instance eq_itree_notauF :
+  Proper (going (@eq_itree E R _ eq) ==> flip impl) notauF.
+Proof.
+  intros ? ? [] ?; punfold H. inv H; simpl in *; subst; eauto.
+Qed.
+
+(* If [t1] and [t2] are equivalent, then either both start with
+   finitely many taus, or both [spin]. *)
+Global Instance euttE_finite_taus :
+  Proper (going euttE ==> flip impl) finite_tausF.
+Proof.
+  intros ? ? [] ?; punfold H. eapply H. eauto.
+Qed.
+
+End EUTT_eq.
+
+(**)
+
+Lemma euttE_tau {E R1 R2} (RR : R1 -> R2 -> Prop)
+           (t1 : itree E R1) (t2 : itree E R2) :
+  euttE RR t1 t2 -> euttE RR (Tau t1) (Tau t2).
+Proof.
+  intros H.
+  pfold. eapply euttEF_tau. reflexivity. reflexivity. punfold H.
+Qed.
+
+Lemma eq_itree_vis {E R1 R2} (RR : R1 -> R2 -> Prop)
+      {U} (e : E U) (k1 : U -> itree E R1) (k2 : U -> itree E R2) :
+  (forall u, eq_itree RR (k1 u) (k2 u)) ->
+  eq_itree RR (Vis e k1) (Vis e k2).
+Proof.
+  intros; pfold; constructor; left. apply H.
+Qed.
+
+Lemma eq_itree_ret {E R1 R2} (RR : R1 -> R2 -> Prop) r1 r2 :
+  RR r1 r2 -> @eq_itree E _ _ RR (Ret r1) (Ret r2).
+Proof.
+  intros; pfold; eauto; constructor; auto.
+Qed.
+
+(* Lemmas about [bind]. *)
+
+Lemma untaus_bind {E S R} : forall t t' (k: S -> itree E R)
+      (UNTAUS: untausF (observe t) (observe t')),
+  untausF (observe (ITree.bind t k)) (observe (ITree.bind t' k)).
+Proof.
+  intros. genobs t ot; genobs t' ot'. revert t Heqot t' Heqot'.
+  induction UNTAUS; intros; subst.
+  - rewrite !unfold_bind; simpobs; eauto.
+  - rewrite unfold_bind. simpobs. cbn. eauto.
+Qed.
+
+Lemma untaus_bindF {E S R} : forall t t' (k: S -> itree E R)
+      (UNTAUS: untausF (observe t) t'),
+  untausF (observe (ITree.bind t k)) (observe (ITree.bind (go t') k)).
+Proof.
+  intros; eapply untaus_bind; eauto.
+Qed.
+
+Lemma finite_taus_bind_fst {E R S}
+      (t : itree E R) (f : R -> itree E S) :
+  finite_taus (ITree.bind t f) -> finite_taus t.
+Proof.
+  intros [tf' [TAUS PROP]].
+  genobs (ITree.bind t f) obtf. move TAUS at top. revert_until TAUS.
+  induction TAUS; intros; subst.
+  - rewrite unfold_bind in PROP.
+    genobs t ot; destruct ot; eauto using finite_taus_ret, finite_taus_vis.
+  - genobs t ot; destruct ot; eauto using finite_taus_ret, finite_taus_vis.
+    rewrite unfold_bind in Heqobtf. simpobs. inv Heqobtf. unfold_bind.
+    eapply finite_taus_tau; eauto.
+Qed.
+
+Lemma finite_taus_bind {E R S}
+      (t : itree E R) (f : R -> itree E S)
+      (FINt: finite_tausF (observe t))
+      (FINk: forall v, finite_tausF (observe (f v))):
+  finite_tausF (observe (ITree.bind t f)).
+Proof.
+  rewrite unfold_bind.
+  genobs t ot. clear Heqot t.
+  destruct FINt as [ot' [UNT NOTAU]].
+  induction UNT; subst.
+  - destruct ot0; inv NOTAU; simpl; eauto 7.
+  - apply finite_taus_tau. eauto.
+Qed.
+
+Inductive euttE_bind_clo {E R1 R2} (r: itree E R1 -> itree E R2 -> Prop) : itree E R1 -> itree E R2 -> Prop :=
+| euttE_bind_clo_intro U (t1 t2: itree E U) k1 k2
+      (EQV: euttE eq t1 t2)
+      (REL: forall v, r (k1 v) (k2 v))
+  : euttE_bind_clo r (ITree.bind t1 k1) (ITree.bind t2 k2)
+.
+Hint Constructors euttE_bind_clo.
+
+Lemma bind_clo_finite_taus {E U R1 R2}  t1 t2 k1 k2
+    (FT: finite_taus (@ITree.bind E U R1 t1 k1))
+    (FTk: forall v, finite_taus (k1 v) -> finite_taus (k2 v))
+    (EQV: euttE eq t1 t2):
+  finite_taus (@ITree.bind E U R2 t2 k2).
+Proof.
+  punfold EQV. destruct EQV as [[FTt _] EQV].
+  assert (FT1 := FT). apply finite_taus_bind_fst in FT1.
+  assert (FT2 := FT1). apply FTt in FT2.
+  destruct FT1 as [a [FT1 NT1]], FT2 as [b [FT2 NT2]].
+  rewrite @untaus_finite_taus in FT; [|eapply untaus_bindF, FT1].
+  rewrite unfold_bind. genobs t2 ot2. clear Heqot2 t2.
+  induction FT2.
+  - destruct ot0; inv NT2; simpl; eauto 7.
+    hexploit EQV; eauto. intros EQV'. inv EQV'.
+    rewrite unfold_bind in FT. eauto.
+  - subst. eapply finite_taus_tau; eauto.
+    eapply IHFT2; eauto using unalltaus_tau'.
+Qed.
+
+Lemma euttE_clo_bind {E R1 R2} RR : weak_respectful2 (@euttE_ E R1 R2 RR) euttE_bind_clo.
+Proof.
+  econstructor; [pmonauto|].
+  intros. destruct PR. split.
+  - assert (EQV':=EQV). symmetry in EQV'.
+    split; intros; eapply bind_clo_finite_taus; eauto; intros.
+    + edestruct GF; eauto. apply FIN. eauto.
+    + edestruct GF; eauto. apply FIN. eauto.
+  - punfold EQV. destruct EQV.
+    intros.
+    hexploit (@finite_taus_bind_fst E); [do 2 eexists; apply UNTAUS1|]. intros [a FT1].
+    hexploit (@finite_taus_bind_fst E); [do 2 eexists; apply UNTAUS2|]. intros [b FT2].
+    specialize (EQV _ _ FT1 FT2).
+    destruct FT1 as [FT1 Hnotau1]. destruct FT2 as [FT2 Hnotau2].
+    hexploit @untaus_bindF; [ eapply FT1 | ]. intros UT1.
+    hexploit @untaus_bindF; [ eapply FT2 | ]. intros UT2.
+    hexploit @untaus_unalltaus_rev; [apply UT1| |]. eauto. intros UAT1.
+    hexploit @untaus_unalltaus_rev; [apply UT2| |]; eauto. intros UAT2.
+    inv EQV.
+    + rewrite unfold_bind in UAT1. rewrite unfold_bind in UAT2. cbn in *.
+      eapply GF in REL. destruct REL.
+      eapply monotone_eq_notauF; eauto using rclo2.
+    + rewrite unfold_bind in UAT1. rewrite unfold_bind in UAT2. cbn in *.
+      destruct UAT1 as [UAT1 _]. destruct UAT2 as [UAT2 _].
+      dependent destruction UAT1. dependent destruction UAT2. simpobs.
+      econstructor. intros. specialize (H x). pclearbot. fold_bind. eauto using rclo2.
+Qed.
+
+Inductive euttE_trans_clo {E R1 R2} (r: itree E R1 -> itree E R2 -> Prop) :
+  itree E R1 -> itree E R2 -> Prop :=
+| euttE_pre_clo_intro t1 t2 t3 t4
+      (EQVl: euttE eq t1 t2)
+      (EQVr: euttE eq t4 t3)
+      (REL: r t2 t3)
+  : euttE_trans_clo r t1 t4
+.
+Hint Constructors euttE_trans_clo.
+
+Lemma euttE_clo_trans {E R1 R2} RR :
+  weak_respectful2 (@euttE_ E R1 R2 RR) euttE_trans_clo.
+Proof.
+  econstructor; [pmonauto|].
+  intros. inv PR.
+  punfold EQVl. punfold EQVr. destruct EQVl, EQVr. split.
+  { rewrite FIN, FIN0. apply GF in REL. destruct REL. eauto. }
+
+  intros. apply proj1 in FIN. edestruct FIN as [n'' [t2'' TAUS'']]; [eexists; eauto|].
+  hexploit EQV; eauto. intros EUTT1.
+  apply proj1 in FIN0. edestruct FIN0 as [n''' [t2''' TAUS''']]; [eexists; eauto|].
+  hexploit EQV0; eauto. intros EUTT2.
+  apply GF in REL. destruct REL.
+  hexploit EQV1; eauto. intros EUTT3.
+  destruct EUTT1; destruct EUTT2;
+    try (solve [subst; inversion EUTT3; auto]).
+  remember (VisF _ _) as o2 in EUTT3.
+  remember (VisF _ _) as o3 in EUTT3.
+  inversion EUTT3; subst; try discriminate.
+  inversion H2; clear H2; inversion H3; clear H3.
+  subst; auto_inj_pair2; subst.
+  econstructor. intros.
+  specialize (H x); specialize (H0 x); specialize (H1 x).
+  pclearbot. eauto using rclo2.
+Qed.
+
+Arguments euttE_clo_trans : clear implicits.
